module minimal {ℓ₁ ℓ₂} (Univ : Set ℓ₁) (⟦_⟧ : Univ → Set ℓ₂)where


open import Function using (id; flip; _∘_)
open import Data.Product using (_×_; _,_)
open import Data.Sum using (_⊎_; inj₁; inj₂)
open import Relation.Nullary using (¬_)
open import Relation.Binary.PropositionalEquality using (_≡_; refl)


infixr  20  _⇒_
infixl  20  _⇐_
infixl  25  _⇚_
infixr  25  _⇛_
infixr  30  _⊗_
infixr  30  _⊕_


data Type : Set ℓ₁ where
  el           : Univ  → Type
  _⊗_ _⇒_ _⇐_  : Type  → Type  → Type
  _⊕_ _⇚_ _⇛_  : Type  → Type  → Type


data Judgement : Set ℓ₁ where
  _⊢_  : Type → Type → Judgement


infix 1 LG_

data LG_ : Judgement → Set ℓ₁ where

  ax   : ∀ {A}       →  LG el A ⊢ el A

  -- residuation and monotonicity for (⇐ , ⊗ , ⇒)
  r⇒⊗  : ∀ {A B C}   →  LG B ⊢ A ⇒ C  → LG A ⊗ B ⊢ C
  r⊗⇒  : ∀ {A B C}   →  LG A ⊗ B ⊢ C  → LG B ⊢ A ⇒ C
  r⇐⊗  : ∀ {A B C}   →  LG A ⊢ C ⇐ B  → LG A ⊗ B ⊢ C
  r⊗⇐  : ∀ {A B C}   →  LG A ⊗ B ⊢ C  → LG A ⊢ C ⇐ B

  m⊗   : ∀ {A B C D} →  LG A ⊢ B      → LG C ⊢ D      → LG A ⊗ C ⊢ B ⊗ D
  m⇒   : ∀ {A B C D} →  LG A ⊢ B      → LG C ⊢ D      → LG B ⇒ C ⊢ A ⇒ D
  m⇐   : ∀ {A B C D} →  LG A ⊢ B      → LG C ⊢ D      → LG A ⇐ D ⊢ B ⇐ C

  -- residuation and monotonicity for (⇚ , ⊕ , ⇛)
  r⇛⊕  : ∀ {A B C}   →  LG B ⇛ C ⊢ A  → LG C ⊢ B ⊕ A
  r⊕⇛  : ∀ {A B C}   →  LG C ⊢ B ⊕ A  → LG B ⇛ C ⊢ A
  r⊕⇚  : ∀ {A B C}   →  LG C ⊢ B ⊕ A  → LG C ⇚ A ⊢ B
  r⇚⊕  : ∀ {A B C}   →  LG C ⇚ A ⊢ B  → LG C ⊢ B ⊕ A

  m⊕   : ∀ {A B C D} →  LG A ⊢ B      → LG C ⊢ D      → LG A ⊕ C ⊢ B ⊕ D
  m⇛   : ∀ {A B C D} →  LG C ⊢ D      → LG A ⊢ B      → LG D ⇛ A ⊢ C ⇛ B
  m⇚   : ∀ {A B C D} →  LG A ⊢ B      → LG C ⊢ D      → LG A ⇚ D ⊢ B ⇚ C

  -- grishin distributives
  d⇛⇐  : ∀ {A B C D} →  LG A ⊗ B ⊢ C ⊕ D  → LG C ⇛ A ⊢ D ⇐ B
  d⇛⇒  : ∀ {A B C D} →  LG A ⊗ B ⊢ C ⊕ D  → LG C ⇛ B ⊢ A ⇒ D
  d⇚⇒  : ∀ {A B C D} →  LG A ⊗ B ⊢ C ⊕ D  → LG B ⇚ D ⊢ A ⇒ C
  d⇚⇐  : ∀ {A B C D} →  LG A ⊗ B ⊢ C ⊕ D  → LG A ⇚ D ⊢ C ⇐ B


ax′ : ∀ {A} → LG A ⊢ A
ax′ {el  _} = ax
ax′ {_ ⊗ _} = m⊗ ax′ ax′
ax′ {_ ⇚ _} = m⇚ ax′ ax′
ax′ {_ ⇛ _} = m⇛ ax′ ax′
ax′ {_ ⊕ _} = m⊕ ax′ ax′
ax′ {_ ⇐ _} = m⇐ ax′ ax′
ax′ {_ ⇒ _} = m⇒ ax′ ax′


appl-⇒′  : ∀ {A B} → LG A ⊗ (A ⇒ B) ⊢ B
appl-⇒′  = r⇒⊗ (m⇒ ax′ ax′)

appl-⇐′  : ∀ {A B} → LG (B ⇐ A) ⊗ A ⊢ B
appl-⇐′  = r⇐⊗ (m⇐ ax′ ax′)

appl-⇛′  : ∀ {A B} → LG B ⊢ A ⊕ (A ⇛ B)
appl-⇛′  = r⇛⊕ (m⇛ ax′ ax′)

appl-⇚′  : ∀ {A B} → LG B ⊢ (B ⇚ A) ⊕ A
appl-⇚′  = r⇚⊕ (m⇚ ax′ ax′)


data Polarity : Set where + -  : Polarity

data Context (p : Polarity) : Polarity → Set ℓ₁ where
  []    : Context p p
  _⊗>_  : Type         → Context p +  → Context p +
  _⇒>_  : Type         → Context p -  → Context p -
  _⇐>_  : Type         → Context p +  → Context p -
  _<⊗_  : Context p +  → Type         → Context p +
  _<⇒_  : Context p +  → Type         → Context p -
  _<⇐_  : Context p -  → Type         → Context p -
  _⊕>_  : Type         → Context p -  → Context p -
  _⇚>_  : Type         → Context p -  → Context p +
  _⇛>_  : Type         → Context p +  → Context p +
  _<⊕_  : Context p -  → Type         → Context p -
  _<⇚_  : Context p +  → Type         → Context p +
  _<⇛_  : Context p -  → Type         → Context p +

data Contextᴶ (p : Polarity) : Set ℓ₁ where
  _<⊢_  : Context p +  → Type         → Contextᴶ p
  _⊢>_  : Type         → Context p -  → Contextᴶ p

_[_] : ∀ {p₁ p₂} → Context p₁ p₂ → Type → Type
[]        [ A ] = A
(B ⊗> C)  [ A ] = B ⊗ (C [ A ])
(C <⊗ B)  [ A ] = (C [ A ]) ⊗ B
(B ⇒> C)  [ A ] = B ⇒ (C [ A ])
(C <⇒ B)  [ A ] = (C [ A ]) ⇒ B
(B ⇐> C)  [ A ] = B ⇐ (C [ A ])
(C <⇐ B)  [ A ] = (C [ A ]) ⇐ B
(B ⊕> C)  [ A ] = B ⊕ (C [ A ])
(C <⊕ B)  [ A ] = (C [ A ]) ⊕ B
(B ⇚> C)  [ A ] = B ⇚ (C [ A ])
(C <⇚ B)  [ A ] = (C [ A ]) ⇚ B
(B ⇛> C)  [ A ] = B ⇛ (C [ A ])
(C <⇛ B)  [ A ] = (C [ A ]) ⇛ B

_[_]ᴶ : ∀ {p} → Contextᴶ p → Type → Judgement
(A <⊢ B) [ C ]ᴶ = A [ C ] ⊢ B
(A ⊢> B) [ C ]ᴶ = A ⊢ B [ C ]


module el where

  data Origin {B} (J : Contextᴶ +) (f : LG J [ el B ]ᴶ) : Set ℓ₁ where
   origin :  (f′  : ∀ {G} → LG G ⊢ el B → LG J [ G ]ᴶ)
             (pr  : f ≡ f′ ax)
                  → Origin J f

  mutual
    find : ∀ {B} (J : Contextᴶ +) (f : LG J [ el B ]ᴶ) → Origin J f
    find ([] <⊢ ._)       ax        = origin id refl
    find ([] <⊢ ._)       (r⊗⇒ f)   = go ((_ ⊗> []) <⊢ _)       f r⊗⇒
    find ([] <⊢ ._)       (r⊗⇐ f)   = go (([] <⊗ _) <⊢ _)       f r⊗⇐
    find ([] <⊢ ._)       (r⇛⊕ f)   = go ((_ ⇛> []) <⊢ _)       f r⇛⊕
    find ([] <⊢ ._)       (r⇚⊕ f)   = go (([] <⇚ _) <⊢ _)       f r⇚⊕
    find ((A ⊗> B) <⊢ ._) (m⊗  f g) = go (B <⊢ _)               g (m⊗ f)
    find ((A ⊗> B) <⊢ ._) (r⇒⊗ f)   = go (B <⊢ _)               f r⇒⊗
    find ((A ⊗> B) <⊢ ._) (r⊗⇒ f)   = go ((_ ⊗> (A ⊗> B)) <⊢ _) f r⊗⇒
    find ((A ⊗> B) <⊢ ._) (r⇐⊗ f)   = go (_ ⊢> (_ ⇐> B))        f r⇐⊗
    find ((A ⊗> B) <⊢ ._) (r⊗⇐ f)   = go (((A ⊗> B) <⊗ _) <⊢ _) f r⊗⇐
    find ((A ⊗> B) <⊢ ._) (r⇛⊕ f)   = go ((_ ⇛> (A ⊗> B)) <⊢ _) f r⇛⊕
    find ((A ⊗> B) <⊢ ._) (r⇚⊕ f)   = go (((A ⊗> B) <⇚ _) <⊢ _) f r⇚⊕
    find ((A ⇛> B) <⊢ ._) (r⊗⇒ f)   = go ((_ ⊗> (A ⇛> B)) <⊢ _) f r⊗⇒
    find ((A ⇛> B) <⊢ ._) (r⊗⇐ f)   = go (((A ⇛> B) <⊗ _) <⊢ _) f r⊗⇐
    find ((A ⇛> B) <⊢ ._) (m⇛  f g) = go (B <⊢ _)               g (m⇛ f)
    find ((A ⇛> B) <⊢ ._) (r⇛⊕ f)   = go ((_ ⇛> (A ⇛> B)) <⊢ _) f r⇛⊕
    find ((A ⇛> B) <⊢ ._) (r⊕⇛ f)   = go (B <⊢ _)               f r⊕⇛
    find ((A ⇛> B) <⊢ ._) (r⇚⊕ f)   = go (((A ⇛> B) <⇚ _) <⊢ _) f r⇚⊕
    find ((A ⇛> B) <⊢ ._) (d⇛⇐ f)   = go ((B <⊗ _) <⊢ _)        f d⇛⇐
    find ((A ⇛> B) <⊢ ._) (d⇛⇒ f)   = go ((_ ⊗> B) <⊢ _)        f d⇛⇒
    find ((A ⇚> B) <⊢ ._) (r⊗⇒ f)   = go ((_ ⊗> (A ⇚> B)) <⊢ _) f r⊗⇒
    find ((A ⇚> B) <⊢ ._) (r⊗⇐ f)   = go (((A ⇚> B) <⊗ _) <⊢ _) f r⊗⇐
    find ((A ⇚> B) <⊢ ._) (m⇚  f g) = go (_ ⊢> B)               g (m⇚ f)
    find ((A ⇚> B) <⊢ ._) (r⇛⊕ f)   = go ((_ ⇛> (A ⇚> B)) <⊢ _) f r⇛⊕
    find ((A ⇚> B) <⊢ ._) (r⊕⇚ f)   = go (_ ⊢> (_ ⊕> B))        f r⊕⇚
    find ((A ⇚> B) <⊢ ._) (r⇚⊕ f)   = go (((A ⇚> B) <⇚ _) <⊢ _) f r⇚⊕
    find ((A ⇚> B) <⊢ ._) (d⇚⇒ f)   = go (_ ⊢> (_ ⊕> B))        f d⇚⇒
    find ((A ⇚> B) <⊢ ._) (d⇚⇐ f)   = go (_ ⊢> (_ ⊕> B))        f d⇚⇐
    find ((A <⊗ B) <⊢ ._) (m⊗  f g) = go (A <⊢ _)               f (flip m⊗ g)
    find ((A <⊗ B) <⊢ ._) (r⇒⊗ f)   = go (_ ⊢> (A <⇒ _))        f r⇒⊗
    find ((A <⊗ B) <⊢ ._) (r⊗⇒ f)   = go ((_ ⊗> (A <⊗ B)) <⊢ _) f r⊗⇒
    find ((A <⊗ B) <⊢ ._) (r⇐⊗ f)   = go (A <⊢ _)               f r⇐⊗
    find ((A <⊗ B) <⊢ ._) (r⊗⇐ f)   = go (((A <⊗ B) <⊗ _) <⊢ _) f r⊗⇐
    find ((A <⊗ B) <⊢ ._) (r⇛⊕ f)   = go ((_ ⇛> (A <⊗ B)) <⊢ _) f r⇛⊕
    find ((A <⊗ B) <⊢ ._) (r⇚⊕ f)   = go (((A <⊗ B) <⇚ _) <⊢ _) f r⇚⊕
    find ((A <⇛ B) <⊢ ._) (r⊗⇒ f)   = go ((_ ⊗> (A <⇛ B)) <⊢ _) f r⊗⇒
    find ((A <⇛ B) <⊢ ._) (r⊗⇐ f)   = go (((A <⇛ B) <⊗ _) <⊢ _) f r⊗⇐
    find ((A <⇛ B) <⊢ ._) (m⇛  f g) = go (_ ⊢> A)               f (flip m⇛ g)
    find ((A <⇛ B) <⊢ ._) (r⇛⊕ f)   = go ((_ ⇛> (A <⇛ B)) <⊢ _) f r⇛⊕
    find ((A <⇛ B) <⊢ ._) (r⊕⇛ f)   = go (_ ⊢> (A <⊕ _))        f r⊕⇛
    find ((A <⇛ B) <⊢ ._) (r⇚⊕ f)   = go (((A <⇛ B) <⇚ _) <⊢ _) f r⇚⊕
    find ((A <⇛ B) <⊢ ._) (d⇛⇐ f)   = go (_ ⊢> (A <⊕ _))        f d⇛⇐
    find ((A <⇛ B) <⊢ ._) (d⇛⇒ f)   = go (_ ⊢> (A <⊕ _))        f d⇛⇒
    find ((A <⇚ B) <⊢ ._) (r⊗⇒ f)   = go ((_ ⊗> (A <⇚ B)) <⊢ _) f r⊗⇒
    find ((A <⇚ B) <⊢ ._) (r⊗⇐ f)   = go (((A <⇚ B) <⊗ _) <⊢ _) f r⊗⇐
    find ((A <⇚ B) <⊢ ._) (m⇚  f g) = go (A <⊢ _)               f (flip m⇚ g)
    find ((A <⇚ B) <⊢ ._) (r⇛⊕ f)   = go ((_ ⇛> (A <⇚ B)) <⊢ _) f r⇛⊕
    find ((A <⇚ B) <⊢ ._) (r⊕⇚ f)   = go (A <⊢ _)               f r⊕⇚
    find ((A <⇚ B) <⊢ ._) (r⇚⊕ f)   = go (((A <⇚ B) <⇚ _) <⊢ _) f r⇚⊕
    find ((A <⇚ B) <⊢ ._) (d⇚⇒ f)   = go ((_ ⊗> A) <⊢ _)        f d⇚⇒
    find ((A <⇚ B) <⊢ ._) (d⇚⇐ f)   = go ((A <⊗ _) <⊢ _)        f d⇚⇐
    find (._ ⊢> (A ⊕> B)) (r⇒⊗ f)   = go (_ ⊢> (_ ⇒> (A ⊕> B))) f r⇒⊗
    find (._ ⊢> (A ⊕> B)) (r⇐⊗ f)   = go (_ ⊢> ((A ⊕> B) <⇐ _)) f r⇐⊗
    find (._ ⊢> (A ⊕> B)) (m⊕  f g) = go (_ ⊢> B)               g (m⊕ f)
    find (._ ⊢> (A ⊕> B)) (r⇛⊕ f)   = go (_ ⊢> B)               f r⇛⊕
    find (._ ⊢> (A ⊕> B)) (r⊕⇛ f)   = go (_ ⊢> (_ ⊕> (A ⊕> B))) f r⊕⇛
    find (._ ⊢> (A ⊕> B)) (r⊕⇚ f)   = go (_ ⊢> ((A ⊕> B) <⊕ _)) f r⊕⇚
    find (._ ⊢> (A ⊕> B)) (r⇚⊕ f)   = go ((_ ⇚> B) <⊢ _)        f r⇚⊕
    find (._ ⊢> (A ⇒> B)) (m⇒  f g) = go (_ ⊢> B)               g (m⇒ f)
    find (._ ⊢> (A ⇒> B)) (r⇒⊗ f)   = go (_ ⊢> (_ ⇒> (A ⇒> B))) f r⇒⊗
    find (._ ⊢> (A ⇒> B)) (r⊗⇒ f)   = go (_ ⊢> B)               f r⊗⇒
    find (._ ⊢> (A ⇒> B)) (r⇐⊗ f)   = go (_ ⊢> ((A ⇒> B) <⇐ _)) f r⇐⊗
    find (._ ⊢> (A ⇒> B)) (r⊕⇛ f)   = go (_ ⊢> (_ ⊕> (A ⇒> B))) f r⊕⇛
    find (._ ⊢> (A ⇒> B)) (r⊕⇚ f)   = go (_ ⊢> ((A ⇒> B) <⊕ _)) f r⊕⇚
    find (._ ⊢> (A ⇒> B)) (d⇛⇒ f)   = go (_ ⊢> (_ ⊕> B))        f d⇛⇒
    find (._ ⊢> (A ⇒> B)) (d⇚⇒ f)   = go (_ ⊢> (B <⊕ _))        f d⇚⇒
    find (._ ⊢> (A ⇐> B)) (m⇐  f g) = go (B <⊢ _)               g (m⇐ f)
    find (._ ⊢> (A ⇐> B)) (r⇒⊗ f)   = go (_ ⊢> (_ ⇒> (A ⇐> B))) f r⇒⊗
    find (._ ⊢> (A ⇐> B)) (r⇐⊗ f)   = go (_ ⊢> ((A ⇐> B) <⇐ _)) f r⇐⊗
    find (._ ⊢> (A ⇐> B)) (r⊗⇐ f)   = go ((_ ⊗> B) <⊢ _)        f r⊗⇐
    find (._ ⊢> (A ⇐> B)) (r⊕⇛ f)   = go (_ ⊢> (_ ⊕> (A ⇐> B))) f r⊕⇛
    find (._ ⊢> (A ⇐> B)) (r⊕⇚ f)   = go (_ ⊢> ((A ⇐> B) <⊕ _)) f r⊕⇚
    find (._ ⊢> (A ⇐> B)) (d⇛⇐ f)   = go ((_ ⊗> B) <⊢ _)        f d⇛⇐
    find (._ ⊢> (A ⇐> B)) (d⇚⇐ f)   = go ((_ ⊗> B) <⊢ _)        f d⇚⇐
    find (._ ⊢> (A <⊕ B)) (r⇒⊗ f)   = go (_ ⊢> (_ ⇒> (A <⊕ B))) f r⇒⊗
    find (._ ⊢> (A <⊕ B)) (r⇐⊗ f)   = go (_ ⊢> ((A <⊕ B) <⇐ _)) f r⇐⊗
    find (._ ⊢> (A <⊕ B)) (m⊕  f g) = go (_ ⊢> A)               f (flip m⊕ g)
    find (._ ⊢> (A <⊕ B)) (r⇛⊕ f)   = go ((A <⇛ _) <⊢ _)        f r⇛⊕
    find (._ ⊢> (A <⊕ B)) (r⊕⇛ f)   = go (_ ⊢> (_ ⊕> (A <⊕ B))) f r⊕⇛
    find (._ ⊢> (A <⊕ B)) (r⊕⇚ f)   = go (_ ⊢> ((A <⊕ B) <⊕ _)) f r⊕⇚
    find (._ ⊢> (A <⊕ B)) (r⇚⊕ f)   = go (_ ⊢> A)               f r⇚⊕
    find (._ ⊢> (A <⇒ B)) (m⇒  f g) = go (A <⊢ _)               f (flip m⇒ g)
    find (._ ⊢> (A <⇒ B)) (r⇒⊗ f)   = go (_ ⊢> (_ ⇒> (A <⇒ B))) f r⇒⊗
    find (._ ⊢> (A <⇒ B)) (r⊗⇒ f)   = go ((A <⊗ _) <⊢ _)        f r⊗⇒
    find (._ ⊢> (A <⇒ B)) (r⇐⊗ f)   = go (_ ⊢> ((A <⇒ B) <⇐ _)) f r⇐⊗
    find (._ ⊢> (A <⇒ B)) (r⊕⇛ f)   = go (_ ⊢> (_ ⊕> (A <⇒ B))) f r⊕⇛
    find (._ ⊢> (A <⇒ B)) (r⊕⇚ f)   = go (_ ⊢> ((A <⇒ B) <⊕ _)) f r⊕⇚
    find (._ ⊢> (A <⇒ B)) (d⇛⇒ f)   = go ((A <⊗ _) <⊢ _)        f d⇛⇒
    find (._ ⊢> (A <⇒ B)) (d⇚⇒ f)   = go ((A <⊗ _) <⊢ _)        f d⇚⇒
    find (._ ⊢> (A <⇐ B)) (m⇐  f g) = go (_ ⊢> A)               f (flip m⇐ g)
    find (._ ⊢> (A <⇐ B)) (r⇒⊗ f)   = go (_ ⊢> (_ ⇒> (A <⇐ B))) f r⇒⊗
    find (._ ⊢> (A <⇐ B)) (r⇐⊗ f)   = go (_ ⊢> ((A <⇐ B) <⇐ _)) f r⇐⊗
    find (._ ⊢> (A <⇐ B)) (r⊗⇐ f)   = go (_ ⊢> A)               f r⊗⇐
    find (._ ⊢> (A <⇐ B)) (r⊕⇛ f)   = go (_ ⊢> (_ ⊕> (A <⇐ B))) f r⊕⇛
    find (._ ⊢> (A <⇐ B)) (r⊕⇚ f)   = go (_ ⊢> ((A <⇐ B) <⊕ _)) f r⊕⇚
    find (._ ⊢> (A <⇐ B)) (d⇛⇐ f)   = go (_ ⊢> (_ ⊕> A))        f d⇛⇐
    find (._ ⊢> (A <⇐ B)) (d⇚⇐ f)   = go (_ ⊢> (A <⊕ _))        f d⇚⇐

    private
      go : ∀ {B}
         → ( I : Contextᴶ + ) (f : LG I [ el B ]ᴶ)
         → { J : Contextᴶ + } (g : ∀ {G} → LG I [ G ]ᴶ → LG J [ G ]ᴶ)
         → Origin J (g f)
      go I x {J} g with find I x
      ... | origin f pr rewrite pr = origin (g ∘ f) refl



module ⊗ where

  data Origin {B C} (J : Contextᴶ -) (f : LG J [ B ⊗ C ]ᴶ) : Set ℓ₁ where
    origin : ∀ {E F}  (h₁  : LG E ⊢ B)
              (h₂  : LG F ⊢ C)
              (f′  : ∀ {G} → LG E ⊗ F ⊢ G → LG J [ G ]ᴶ)
              (pr  : f ≡ f′ (m⊗ h₁ h₂))
                   → Origin J f

  mutual
    find : ∀ {B C} (J : Contextᴶ -) (f : LG J [ B ⊗ C ]ᴶ) → Origin J f
    find (._ ⊢> [])       (m⊗  f g) = origin f g id refl
    find (._ ⊢> [])       (r⇒⊗ f)   = go (_ ⊢> (_ ⇒> []))       f r⇒⊗
    find (._ ⊢> [])       (r⇐⊗ f)   = go (_ ⊢> ([] <⇐ _))       f r⇐⊗
    find (._ ⊢> [])       (r⊕⇛ f)   = go (_ ⊢> (_ ⊕> []))       f r⊕⇛
    find (._ ⊢> [])       (r⊕⇚ f)   = go (_ ⊢> ([] <⊕ _))       f r⊕⇚
    find ((A ⊗> B) <⊢ ._) (m⊗  f g) = go (B <⊢ _)               g (m⊗ f)
    find ((A ⊗> B) <⊢ ._) (r⇒⊗ f)   = go (B <⊢ _)               f r⇒⊗
    find ((A ⊗> B) <⊢ ._) (r⊗⇒ f)   = go ((_ ⊗> (A ⊗> B)) <⊢ _) f r⊗⇒
    find ((A ⊗> B) <⊢ ._) (r⇐⊗ f)   = go (_ ⊢> (_ ⇐> B))        f r⇐⊗
    find ((A ⊗> B) <⊢ ._) (r⊗⇐ f)   = go (((A ⊗> B) <⊗ _) <⊢ _) f r⊗⇐
    find ((A ⊗> B) <⊢ ._) (r⇛⊕ f)   = go ((_ ⇛> (A ⊗> B)) <⊢ _) f r⇛⊕
    find ((A ⊗> B) <⊢ ._) (r⇚⊕ f)   = go (((A ⊗> B) <⇚ _) <⊢ _) f r⇚⊕
    find ((A ⇛> B) <⊢ ._) (r⊗⇒ f)   = go ((_ ⊗> (A ⇛> B)) <⊢ _) f r⊗⇒
    find ((A ⇛> B) <⊢ ._) (r⊗⇐ f)   = go (((A ⇛> B) <⊗ _) <⊢ _) f r⊗⇐
    find ((A ⇛> B) <⊢ ._) (m⇛  f g) = go (B <⊢ _)               g (m⇛ f)
    find ((A ⇛> B) <⊢ ._) (r⇛⊕ f)   = go ((_ ⇛> (A ⇛> B)) <⊢ _) f r⇛⊕
    find ((A ⇛> B) <⊢ ._) (r⊕⇛ f)   = go (B <⊢ _)               f r⊕⇛
    find ((A ⇛> B) <⊢ ._) (r⇚⊕ f)   = go (((A ⇛> B) <⇚ _) <⊢ _) f r⇚⊕
    find ((A ⇛> B) <⊢ ._) (d⇛⇐ f)   = go ((B <⊗ _) <⊢ _)        f d⇛⇐
    find ((A ⇛> B) <⊢ ._) (d⇛⇒ f)   = go ((_ ⊗> B) <⊢ _)        f d⇛⇒
    find ((A ⇚> B) <⊢ ._) (r⊗⇒ f)   = go ((_ ⊗> (A ⇚> B)) <⊢ _) f r⊗⇒
    find ((A ⇚> B) <⊢ ._) (r⊗⇐ f)   = go (((A ⇚> B) <⊗ _) <⊢ _) f r⊗⇐
    find ((A ⇚> B) <⊢ ._) (m⇚  f g) = go (_ ⊢> B)               g (m⇚ f)
    find ((A ⇚> B) <⊢ ._) (r⇛⊕ f)   = go ((_ ⇛> (A ⇚> B)) <⊢ _) f r⇛⊕
    find ((A ⇚> B) <⊢ ._) (r⊕⇚ f)   = go (_ ⊢> (_ ⊕> B))        f r⊕⇚
    find ((A ⇚> B) <⊢ ._) (r⇚⊕ f)   = go (((A ⇚> B) <⇚ _) <⊢ _) f r⇚⊕
    find ((A ⇚> B) <⊢ ._) (d⇚⇒ f)   = go (_ ⊢> (_ ⊕> B))        f d⇚⇒
    find ((A ⇚> B) <⊢ ._) (d⇚⇐ f)   = go (_ ⊢> (_ ⊕> B))        f d⇚⇐
    find ((A <⊗ B) <⊢ ._) (m⊗  f g) = go (A <⊢ _)               f (flip m⊗ g)
    find ((A <⊗ B) <⊢ ._) (r⇒⊗ f)   = go (_ ⊢> (A <⇒ _))        f r⇒⊗
    find ((A <⊗ B) <⊢ ._) (r⊗⇒ f)   = go ((_ ⊗> (A <⊗ B)) <⊢ _) f r⊗⇒
    find ((A <⊗ B) <⊢ ._) (r⇐⊗ f)   = go (A <⊢ _)               f r⇐⊗
    find ((A <⊗ B) <⊢ ._) (r⊗⇐ f)   = go (((A <⊗ B) <⊗ _) <⊢ _) f r⊗⇐
    find ((A <⊗ B) <⊢ ._) (r⇛⊕ f)   = go ((_ ⇛> (A <⊗ B)) <⊢ _) f r⇛⊕
    find ((A <⊗ B) <⊢ ._) (r⇚⊕ f)   = go (((A <⊗ B) <⇚ _) <⊢ _) f r⇚⊕
    find ((A <⇛ B) <⊢ ._) (r⊗⇒ f)   = go ((_ ⊗> (A <⇛ B)) <⊢ _) f r⊗⇒
    find ((A <⇛ B) <⊢ ._) (r⊗⇐ f)   = go (((A <⇛ B) <⊗ _) <⊢ _) f r⊗⇐
    find ((A <⇛ B) <⊢ ._) (m⇛  f g) = go (_ ⊢> A)               f (flip m⇛ g)
    find ((A <⇛ B) <⊢ ._) (r⇛⊕ f)   = go ((_ ⇛> (A <⇛ B)) <⊢ _) f r⇛⊕
    find ((A <⇛ B) <⊢ ._) (r⊕⇛ f)   = go (_ ⊢> (A <⊕ _))        f r⊕⇛
    find ((A <⇛ B) <⊢ ._) (r⇚⊕ f)   = go (((A <⇛ B) <⇚ _) <⊢ _) f r⇚⊕
    find ((A <⇛ B) <⊢ ._) (d⇛⇐ f)   = go (_ ⊢> (A <⊕ _))        f d⇛⇐
    find ((A <⇛ B) <⊢ ._) (d⇛⇒ f)   = go (_ ⊢> (A <⊕ _))        f d⇛⇒
    find ((A <⇚ B) <⊢ ._) (r⊗⇒ f)   = go ((_ ⊗> (A <⇚ B)) <⊢ _) f r⊗⇒
    find ((A <⇚ B) <⊢ ._) (r⊗⇐ f)   = go (((A <⇚ B) <⊗ _) <⊢ _) f r⊗⇐
    find ((A <⇚ B) <⊢ ._) (m⇚  f g) = go (A <⊢ _)               f (flip m⇚ g)
    find ((A <⇚ B) <⊢ ._) (r⇛⊕ f)   = go ((_ ⇛> (A <⇚ B)) <⊢ _) f r⇛⊕
    find ((A <⇚ B) <⊢ ._) (r⊕⇚ f)   = go (A <⊢ _)               f r⊕⇚
    find ((A <⇚ B) <⊢ ._) (r⇚⊕ f)   = go (((A <⇚ B) <⇚ _) <⊢ _) f r⇚⊕
    find ((A <⇚ B) <⊢ ._) (d⇚⇒ f)   = go ((_ ⊗> A) <⊢ _)        f d⇚⇒
    find ((A <⇚ B) <⊢ ._) (d⇚⇐ f)   = go ((A <⊗ _) <⊢ _)        f d⇚⇐
    find (._ ⊢> (A ⊕> B)) (r⇒⊗ f)   = go (_ ⊢> (_ ⇒> (A ⊕> B))) f r⇒⊗
    find (._ ⊢> (A ⊕> B)) (r⇐⊗ f)   = go (_ ⊢> ((A ⊕> B) <⇐ _)) f r⇐⊗
    find (._ ⊢> (A ⊕> B)) (m⊕  f g) = go (_ ⊢> B)               g (m⊕ f)
    find (._ ⊢> (A ⊕> B)) (r⇛⊕ f)   = go (_ ⊢> B)               f r⇛⊕
    find (._ ⊢> (A ⊕> B)) (r⊕⇛ f)   = go (_ ⊢> (_ ⊕> (A ⊕> B))) f r⊕⇛
    find (._ ⊢> (A ⊕> B)) (r⊕⇚ f)   = go (_ ⊢> ((A ⊕> B) <⊕ _)) f r⊕⇚
    find (._ ⊢> (A ⊕> B)) (r⇚⊕ f)   = go ((_ ⇚> B) <⊢ _)        f r⇚⊕
    find (._ ⊢> (A ⇒> B)) (m⇒  f g) = go (_ ⊢> B)               g (m⇒ f)
    find (._ ⊢> (A ⇒> B)) (r⇒⊗ f)   = go (_ ⊢> (_ ⇒> (A ⇒> B))) f r⇒⊗
    find (._ ⊢> (A ⇒> B)) (r⊗⇒ f)   = go (_ ⊢> B)               f r⊗⇒
    find (._ ⊢> (A ⇒> B)) (r⇐⊗ f)   = go (_ ⊢> ((A ⇒> B) <⇐ _)) f r⇐⊗
    find (._ ⊢> (A ⇒> B)) (r⊕⇛ f)   = go (_ ⊢> (_ ⊕> (A ⇒> B))) f r⊕⇛
    find (._ ⊢> (A ⇒> B)) (r⊕⇚ f)   = go (_ ⊢> ((A ⇒> B) <⊕ _)) f r⊕⇚
    find (._ ⊢> (A ⇒> B)) (d⇛⇒ f)   = go (_ ⊢> (_ ⊕> B))        f d⇛⇒
    find (._ ⊢> (A ⇒> B)) (d⇚⇒ f)   = go (_ ⊢> (B <⊕ _))        f d⇚⇒
    find (._ ⊢> (A ⇐> B)) (m⇐  f g) = go (B <⊢ _)               g (m⇐ f)
    find (._ ⊢> (A ⇐> B)) (r⇒⊗ f)   = go (_ ⊢> (_ ⇒> (A ⇐> B))) f r⇒⊗
    find (._ ⊢> (A ⇐> B)) (r⇐⊗ f)   = go (_ ⊢> ((A ⇐> B) <⇐ _)) f r⇐⊗
    find (._ ⊢> (A ⇐> B)) (r⊗⇐ f)   = go ((_ ⊗> B) <⊢ _)        f r⊗⇐
    find (._ ⊢> (A ⇐> B)) (r⊕⇛ f)   = go (_ ⊢> (_ ⊕> (A ⇐> B))) f r⊕⇛
    find (._ ⊢> (A ⇐> B)) (r⊕⇚ f)   = go (_ ⊢> ((A ⇐> B) <⊕ _)) f r⊕⇚
    find (._ ⊢> (A ⇐> B)) (d⇛⇐ f)   = go ((_ ⊗> B) <⊢ _)        f d⇛⇐
    find (._ ⊢> (A ⇐> B)) (d⇚⇐ f)   = go ((_ ⊗> B) <⊢ _)        f d⇚⇐
    find (._ ⊢> (A <⊕ B)) (r⇒⊗ f)   = go (_ ⊢> (_ ⇒> (A <⊕ B))) f r⇒⊗
    find (._ ⊢> (A <⊕ B)) (r⇐⊗ f)   = go (_ ⊢> ((A <⊕ B) <⇐ _)) f r⇐⊗
    find (._ ⊢> (A <⊕ B)) (m⊕  f g) = go (_ ⊢> A)               f (flip m⊕ g)
    find (._ ⊢> (A <⊕ B)) (r⇛⊕ f)   = go ((A <⇛ _) <⊢ _)        f r⇛⊕
    find (._ ⊢> (A <⊕ B)) (r⊕⇛ f)   = go (_ ⊢> (_ ⊕> (A <⊕ B))) f r⊕⇛
    find (._ ⊢> (A <⊕ B)) (r⊕⇚ f)   = go (_ ⊢> ((A <⊕ B) <⊕ _)) f r⊕⇚
    find (._ ⊢> (A <⊕ B)) (r⇚⊕ f)   = go (_ ⊢> A)               f r⇚⊕
    find (._ ⊢> (A <⇒ B)) (m⇒  f g) = go (A <⊢ _)               f (flip m⇒ g)
    find (._ ⊢> (A <⇒ B)) (r⇒⊗ f)   = go (_ ⊢> (_ ⇒> (A <⇒ B))) f r⇒⊗
    find (._ ⊢> (A <⇒ B)) (r⊗⇒ f)   = go ((A <⊗ _) <⊢ _)        f r⊗⇒
    find (._ ⊢> (A <⇒ B)) (r⇐⊗ f)   = go (_ ⊢> ((A <⇒ B) <⇐ _)) f r⇐⊗
    find (._ ⊢> (A <⇒ B)) (r⊕⇛ f)   = go (_ ⊢> (_ ⊕> (A <⇒ B))) f r⊕⇛
    find (._ ⊢> (A <⇒ B)) (r⊕⇚ f)   = go (_ ⊢> ((A <⇒ B) <⊕ _)) f r⊕⇚
    find (._ ⊢> (A <⇒ B)) (d⇛⇒ f)   = go ((A <⊗ _) <⊢ _)        f d⇛⇒
    find (._ ⊢> (A <⇒ B)) (d⇚⇒ f)   = go ((A <⊗ _) <⊢ _)        f d⇚⇒
    find (._ ⊢> (A <⇐ B)) (m⇐  f g) = go (_ ⊢> A)               f (flip m⇐ g)
    find (._ ⊢> (A <⇐ B)) (r⇒⊗ f)   = go (_ ⊢> (_ ⇒> (A <⇐ B))) f r⇒⊗
    find (._ ⊢> (A <⇐ B)) (r⇐⊗ f)   = go (_ ⊢> ((A <⇐ B) <⇐ _)) f r⇐⊗
    find (._ ⊢> (A <⇐ B)) (r⊗⇐ f)   = go (_ ⊢> A)               f r⊗⇐
    find (._ ⊢> (A <⇐ B)) (r⊕⇛ f)   = go (_ ⊢> (_ ⊕> (A <⇐ B))) f r⊕⇛
    find (._ ⊢> (A <⇐ B)) (r⊕⇚ f)   = go (_ ⊢> ((A <⇐ B) <⊕ _)) f r⊕⇚
    find (._ ⊢> (A <⇐ B)) (d⇛⇐ f)   = go (_ ⊢> (_ ⊕> A))        f d⇛⇐
    find (._ ⊢> (A <⇐ B)) (d⇚⇐ f)   = go (_ ⊢> (A <⊕ _))        f d⇚⇐

    private
      go : ∀ {B C}
         → ( I : Contextᴶ - ) (f : LG I [ B ⊗ C ]ᴶ)
         → { J : Contextᴶ - } (g : ∀ {G} → LG I [ G ]ᴶ → LG J [ G ]ᴶ)
         → Origin J (g f)
      go I f {J} g with find I f
      ... | origin h₁ h₂ f′ pr rewrite pr = origin h₁ h₂ (g ∘ f′) refl



module ⇒ where

  data Origin {B C} (J : Contextᴶ +) (f : LG J [ B ⇒ C ]ᴶ) : Set ℓ₁ where
    origin : ∀ {E F}  (h₁  : LG E ⊢ B)
              (h₂  : LG C ⊢ F)
              (f′  : ∀ {G} → LG G ⊢ E ⇒ F → LG J [ G ]ᴶ)
              (pr  : f ≡ f′ (m⇒ h₁ h₂))
                   → Origin J f

  mutual
    find : ∀ {B C} (J : Contextᴶ +) (f : LG J [ B ⇒ C ]ᴶ) → Origin J f
    find ([] <⊢ ._)       (m⇒  f g) = origin f g id refl
    find ([] <⊢ ._)       (r⊗⇒ f)   = go ((_ ⊗> []) <⊢ _)       f r⊗⇒
    find ([] <⊢ ._)       (r⊗⇐ f)   = go (([] <⊗ _) <⊢ _)       f r⊗⇐
    find ([] <⊢ ._)       (r⇛⊕ f)   = go ((_ ⇛> []) <⊢ _)       f r⇛⊕
    find ([] <⊢ ._)       (r⇚⊕ f)   = go (([] <⇚ _) <⊢ _)       f r⇚⊕
    find ((A ⊗> B) <⊢ ._) (m⊗  f g) = go (B <⊢ _)               g (m⊗ f)
    find ((A ⊗> B) <⊢ ._) (r⇒⊗ f)   = go (B <⊢ _)               f r⇒⊗
    find ((A ⊗> B) <⊢ ._) (r⊗⇒ f)   = go ((_ ⊗> (A ⊗> B)) <⊢ _) f r⊗⇒
    find ((A ⊗> B) <⊢ ._) (r⇐⊗ f)   = go (_ ⊢> (_ ⇐> B))        f r⇐⊗
    find ((A ⊗> B) <⊢ ._) (r⊗⇐ f)   = go (((A ⊗> B) <⊗ _) <⊢ _) f r⊗⇐
    find ((A ⊗> B) <⊢ ._) (r⇛⊕ f)   = go ((_ ⇛> (A ⊗> B)) <⊢ _) f r⇛⊕
    find ((A ⊗> B) <⊢ ._) (r⇚⊕ f)   = go (((A ⊗> B) <⇚ _) <⊢ _) f r⇚⊕
    find ((A ⇛> B) <⊢ ._) (r⊗⇒ f)   = go ((_ ⊗> (A ⇛> B)) <⊢ _) f r⊗⇒
    find ((A ⇛> B) <⊢ ._) (r⊗⇐ f)   = go (((A ⇛> B) <⊗ _) <⊢ _) f r⊗⇐
    find ((A ⇛> B) <⊢ ._) (m⇛  f g) = go (B <⊢ _)               g (m⇛ f)
    find ((A ⇛> B) <⊢ ._) (r⇛⊕ f)   = go ((_ ⇛> (A ⇛> B)) <⊢ _) f r⇛⊕
    find ((A ⇛> B) <⊢ ._) (r⊕⇛ f)   = go (B <⊢ _)               f r⊕⇛
    find ((A ⇛> B) <⊢ ._) (r⇚⊕ f)   = go (((A ⇛> B) <⇚ _) <⊢ _) f r⇚⊕
    find ((A ⇛> B) <⊢ ._) (d⇛⇐ f)   = go ((B <⊗ _) <⊢ _)        f d⇛⇐
    find ((A ⇛> B) <⊢ ._) (d⇛⇒ f)   = go ((_ ⊗> B) <⊢ _)        f d⇛⇒
    find ((A ⇚> B) <⊢ ._) (r⊗⇒ f)   = go ((_ ⊗> (A ⇚> B)) <⊢ _) f r⊗⇒
    find ((A ⇚> B) <⊢ ._) (r⊗⇐ f)   = go (((A ⇚> B) <⊗ _) <⊢ _) f r⊗⇐
    find ((A ⇚> B) <⊢ ._) (m⇚  f g) = go (_ ⊢> B)               g (m⇚ f)
    find ((A ⇚> B) <⊢ ._) (r⇛⊕ f)   = go ((_ ⇛> (A ⇚> B)) <⊢ _) f r⇛⊕
    find ((A ⇚> B) <⊢ ._) (r⊕⇚ f)   = go (_ ⊢> (_ ⊕> B))        f r⊕⇚
    find ((A ⇚> B) <⊢ ._) (r⇚⊕ f)   = go (((A ⇚> B) <⇚ _) <⊢ _) f r⇚⊕
    find ((A ⇚> B) <⊢ ._) (d⇚⇒ f)   = go (_ ⊢> (_ ⊕> B))        f d⇚⇒
    find ((A ⇚> B) <⊢ ._) (d⇚⇐ f)   = go (_ ⊢> (_ ⊕> B))        f d⇚⇐
    find ((A <⊗ B) <⊢ ._) (m⊗  f g) = go (A <⊢ _)               f (flip m⊗ g)
    find ((A <⊗ B) <⊢ ._) (r⇒⊗ f)   = go (_ ⊢> (A <⇒ _))        f r⇒⊗
    find ((A <⊗ B) <⊢ ._) (r⊗⇒ f)   = go ((_ ⊗> (A <⊗ B)) <⊢ _) f r⊗⇒
    find ((A <⊗ B) <⊢ ._) (r⇐⊗ f)   = go (A <⊢ _)               f r⇐⊗
    find ((A <⊗ B) <⊢ ._) (r⊗⇐ f)   = go (((A <⊗ B) <⊗ _) <⊢ _) f r⊗⇐
    find ((A <⊗ B) <⊢ ._) (r⇛⊕ f)   = go ((_ ⇛> (A <⊗ B)) <⊢ _) f r⇛⊕
    find ((A <⊗ B) <⊢ ._) (r⇚⊕ f)   = go (((A <⊗ B) <⇚ _) <⊢ _) f r⇚⊕
    find ((A <⇛ B) <⊢ ._) (r⊗⇒ f)   = go ((_ ⊗> (A <⇛ B)) <⊢ _) f r⊗⇒
    find ((A <⇛ B) <⊢ ._) (r⊗⇐ f)   = go (((A <⇛ B) <⊗ _) <⊢ _) f r⊗⇐
    find ((A <⇛ B) <⊢ ._) (m⇛  f g) = go (_ ⊢> A)               f (flip m⇛ g)
    find ((A <⇛ B) <⊢ ._) (r⇛⊕ f)   = go ((_ ⇛> (A <⇛ B)) <⊢ _) f r⇛⊕
    find ((A <⇛ B) <⊢ ._) (r⊕⇛ f)   = go (_ ⊢> (A <⊕ _))        f r⊕⇛
    find ((A <⇛ B) <⊢ ._) (r⇚⊕ f)   = go (((A <⇛ B) <⇚ _) <⊢ _) f r⇚⊕
    find ((A <⇛ B) <⊢ ._) (d⇛⇐ f)   = go (_ ⊢> (A <⊕ _))        f d⇛⇐
    find ((A <⇛ B) <⊢ ._) (d⇛⇒ f)   = go (_ ⊢> (A <⊕ _))        f d⇛⇒
    find ((A <⇚ B) <⊢ ._) (r⊗⇒ f)   = go ((_ ⊗> (A <⇚ B)) <⊢ _) f r⊗⇒
    find ((A <⇚ B) <⊢ ._) (r⊗⇐ f)   = go (((A <⇚ B) <⊗ _) <⊢ _) f r⊗⇐
    find ((A <⇚ B) <⊢ ._) (m⇚  f g) = go (A <⊢ _)               f (flip m⇚ g)
    find ((A <⇚ B) <⊢ ._) (r⇛⊕ f)   = go ((_ ⇛> (A <⇚ B)) <⊢ _) f r⇛⊕
    find ((A <⇚ B) <⊢ ._) (r⊕⇚ f)   = go (A <⊢ _)               f r⊕⇚
    find ((A <⇚ B) <⊢ ._) (r⇚⊕ f)   = go (((A <⇚ B) <⇚ _) <⊢ _) f r⇚⊕
    find ((A <⇚ B) <⊢ ._) (d⇚⇒ f)   = go ((_ ⊗> A) <⊢ _)        f d⇚⇒
    find ((A <⇚ B) <⊢ ._) (d⇚⇐ f)   = go ((A <⊗ _) <⊢ _)        f d⇚⇐
    find (._ ⊢> (A ⊕> B)) (r⇒⊗ f)   = go (_ ⊢> (_ ⇒> (A ⊕> B))) f r⇒⊗
    find (._ ⊢> (A ⊕> B)) (r⇐⊗ f)   = go (_ ⊢> ((A ⊕> B) <⇐ _)) f r⇐⊗
    find (._ ⊢> (A ⊕> B)) (m⊕  f g) = go (_ ⊢> B)               g (m⊕ f)
    find (._ ⊢> (A ⊕> B)) (r⇛⊕ f)   = go (_ ⊢> B)               f r⇛⊕
    find (._ ⊢> (A ⊕> B)) (r⊕⇛ f)   = go (_ ⊢> (_ ⊕> (A ⊕> B))) f r⊕⇛
    find (._ ⊢> (A ⊕> B)) (r⊕⇚ f)   = go (_ ⊢> ((A ⊕> B) <⊕ _)) f r⊕⇚
    find (._ ⊢> (A ⊕> B)) (r⇚⊕ f)   = go ((_ ⇚> B) <⊢ _)        f r⇚⊕
    find (._ ⊢> (A ⇒> B)) (m⇒  f g) = go (_ ⊢> B)               g (m⇒ f)
    find (._ ⊢> (A ⇒> B)) (r⇒⊗ f)   = go (_ ⊢> (_ ⇒> (A ⇒> B))) f r⇒⊗
    find (._ ⊢> (A ⇒> B)) (r⊗⇒ f)   = go (_ ⊢> B)               f r⊗⇒
    find (._ ⊢> (A ⇒> B)) (r⇐⊗ f)   = go (_ ⊢> ((A ⇒> B) <⇐ _)) f r⇐⊗
    find (._ ⊢> (A ⇒> B)) (r⊕⇛ f)   = go (_ ⊢> (_ ⊕> (A ⇒> B))) f r⊕⇛
    find (._ ⊢> (A ⇒> B)) (r⊕⇚ f)   = go (_ ⊢> ((A ⇒> B) <⊕ _)) f r⊕⇚
    find (._ ⊢> (A ⇒> B)) (d⇛⇒ f)   = go (_ ⊢> (_ ⊕> B))        f d⇛⇒
    find (._ ⊢> (A ⇒> B)) (d⇚⇒ f)   = go (_ ⊢> (B <⊕ _))        f d⇚⇒
    find (._ ⊢> (A ⇐> B)) (m⇐  f g) = go (B <⊢ _)               g (m⇐ f)
    find (._ ⊢> (A ⇐> B)) (r⇒⊗ f)   = go (_ ⊢> (_ ⇒> (A ⇐> B))) f r⇒⊗
    find (._ ⊢> (A ⇐> B)) (r⇐⊗ f)   = go (_ ⊢> ((A ⇐> B) <⇐ _)) f r⇐⊗
    find (._ ⊢> (A ⇐> B)) (r⊗⇐ f)   = go ((_ ⊗> B) <⊢ _)        f r⊗⇐
    find (._ ⊢> (A ⇐> B)) (r⊕⇛ f)   = go (_ ⊢> (_ ⊕> (A ⇐> B))) f r⊕⇛
    find (._ ⊢> (A ⇐> B)) (r⊕⇚ f)   = go (_ ⊢> ((A ⇐> B) <⊕ _)) f r⊕⇚
    find (._ ⊢> (A ⇐> B)) (d⇛⇐ f)   = go ((_ ⊗> B) <⊢ _)        f d⇛⇐
    find (._ ⊢> (A ⇐> B)) (d⇚⇐ f)   = go ((_ ⊗> B) <⊢ _)        f d⇚⇐
    find (._ ⊢> (A <⊕ B)) (r⇒⊗ f)   = go (_ ⊢> (_ ⇒> (A <⊕ B))) f r⇒⊗
    find (._ ⊢> (A <⊕ B)) (r⇐⊗ f)   = go (_ ⊢> ((A <⊕ B) <⇐ _)) f r⇐⊗
    find (._ ⊢> (A <⊕ B)) (m⊕  f g) = go (_ ⊢> A)               f (flip m⊕ g)
    find (._ ⊢> (A <⊕ B)) (r⇛⊕ f)   = go ((A <⇛ _) <⊢ _)        f r⇛⊕
    find (._ ⊢> (A <⊕ B)) (r⊕⇛ f)   = go (_ ⊢> (_ ⊕> (A <⊕ B))) f r⊕⇛
    find (._ ⊢> (A <⊕ B)) (r⊕⇚ f)   = go (_ ⊢> ((A <⊕ B) <⊕ _)) f r⊕⇚
    find (._ ⊢> (A <⊕ B)) (r⇚⊕ f)   = go (_ ⊢> A)               f r⇚⊕
    find (._ ⊢> (A <⇒ B)) (m⇒  f g) = go (A <⊢ _)               f (flip m⇒ g)
    find (._ ⊢> (A <⇒ B)) (r⇒⊗ f)   = go (_ ⊢> (_ ⇒> (A <⇒ B))) f r⇒⊗
    find (._ ⊢> (A <⇒ B)) (r⊗⇒ f)   = go ((A <⊗ _) <⊢ _)        f r⊗⇒
    find (._ ⊢> (A <⇒ B)) (r⇐⊗ f)   = go (_ ⊢> ((A <⇒ B) <⇐ _)) f r⇐⊗
    find (._ ⊢> (A <⇒ B)) (r⊕⇛ f)   = go (_ ⊢> (_ ⊕> (A <⇒ B))) f r⊕⇛
    find (._ ⊢> (A <⇒ B)) (r⊕⇚ f)   = go (_ ⊢> ((A <⇒ B) <⊕ _)) f r⊕⇚
    find (._ ⊢> (A <⇒ B)) (d⇛⇒ f)   = go ((A <⊗ _) <⊢ _)        f d⇛⇒
    find (._ ⊢> (A <⇒ B)) (d⇚⇒ f)   = go ((A <⊗ _) <⊢ _)        f d⇚⇒
    find (._ ⊢> (A <⇐ B)) (m⇐  f g) = go (_ ⊢> A)               f (flip m⇐ g)
    find (._ ⊢> (A <⇐ B)) (r⇒⊗ f)   = go (_ ⊢> (_ ⇒> (A <⇐ B))) f r⇒⊗
    find (._ ⊢> (A <⇐ B)) (r⇐⊗ f)   = go (_ ⊢> ((A <⇐ B) <⇐ _)) f r⇐⊗
    find (._ ⊢> (A <⇐ B)) (r⊗⇐ f)   = go (_ ⊢> A)               f r⊗⇐
    find (._ ⊢> (A <⇐ B)) (r⊕⇛ f)   = go (_ ⊢> (_ ⊕> (A <⇐ B))) f r⊕⇛
    find (._ ⊢> (A <⇐ B)) (r⊕⇚ f)   = go (_ ⊢> ((A <⇐ B) <⊕ _)) f r⊕⇚
    find (._ ⊢> (A <⇐ B)) (d⇛⇐ f)   = go (_ ⊢> (_ ⊕> A))        f d⇛⇐
    find (._ ⊢> (A <⇐ B)) (d⇚⇐ f)   = go (_ ⊢> (A <⊕ _))        f d⇚⇐

    private
      go : ∀ {B C}
         → ( I : Contextᴶ + ) (f : LG I [ B ⇒ C ]ᴶ)
         → { J : Contextᴶ + } (g : ∀ {G} → LG I [ G ]ᴶ → LG J [ G ]ᴶ)
         → Origin J (g f)
      go I f {J} g with find I f
      ... | origin h₁ h₂ f′ pr rewrite pr = origin h₁ h₂ (g ∘ f′) refl


module ⇐ where

  data Origin {B C} (J : Contextᴶ +) (f : LG J [ B ⇐ C ]ᴶ) : Set ℓ₁ where
    origin : ∀ {E F}  (h₁  : LG B ⊢ E)
              (h₂  : LG F ⊢ C)
              (f′  : ∀ {G} → LG G ⊢ E ⇐ F → LG J [ G ]ᴶ)
              (pr  : f ≡ f′ (m⇐ h₁ h₂))
                   → Origin J f

  mutual
    find : ∀ {B C} (J : Contextᴶ +) (f : LG J [ B ⇐ C ]ᴶ) → Origin J f
    find ([] <⊢ ._)       (m⇐  f g) = origin f g id refl
    find ([] <⊢ ._)       (r⊗⇒ f)   = go ((_ ⊗> []) <⊢ _)       f r⊗⇒
    find ([] <⊢ ._)       (r⊗⇐ f)   = go (([] <⊗ _) <⊢ _)       f r⊗⇐
    find ([] <⊢ ._)       (r⇛⊕ f)   = go ((_ ⇛> []) <⊢ _)       f r⇛⊕
    find ([] <⊢ ._)       (r⇚⊕ f)   = go (([] <⇚ _) <⊢ _)       f r⇚⊕
    find ((A ⊗> B) <⊢ ._) (m⊗  f g) = go (B <⊢ _)               g (m⊗ f)
    find ((A ⊗> B) <⊢ ._) (r⇒⊗ f)   = go (B <⊢ _)               f r⇒⊗
    find ((A ⊗> B) <⊢ ._) (r⊗⇒ f)   = go ((_ ⊗> (A ⊗> B)) <⊢ _) f r⊗⇒
    find ((A ⊗> B) <⊢ ._) (r⇐⊗ f)   = go (_ ⊢> (_ ⇐> B))        f r⇐⊗
    find ((A ⊗> B) <⊢ ._) (r⊗⇐ f)   = go (((A ⊗> B) <⊗ _) <⊢ _) f r⊗⇐
    find ((A ⊗> B) <⊢ ._) (r⇛⊕ f)   = go ((_ ⇛> (A ⊗> B)) <⊢ _) f r⇛⊕
    find ((A ⊗> B) <⊢ ._) (r⇚⊕ f)   = go (((A ⊗> B) <⇚ _) <⊢ _) f r⇚⊕
    find ((A ⇛> B) <⊢ ._) (r⊗⇒ f)   = go ((_ ⊗> (A ⇛> B)) <⊢ _) f r⊗⇒
    find ((A ⇛> B) <⊢ ._) (r⊗⇐ f)   = go (((A ⇛> B) <⊗ _) <⊢ _) f r⊗⇐
    find ((A ⇛> B) <⊢ ._) (m⇛  f g) = go (B <⊢ _)               g (m⇛ f)
    find ((A ⇛> B) <⊢ ._) (r⇛⊕ f)   = go ((_ ⇛> (A ⇛> B)) <⊢ _) f r⇛⊕
    find ((A ⇛> B) <⊢ ._) (r⊕⇛ f)   = go (B <⊢ _)               f r⊕⇛
    find ((A ⇛> B) <⊢ ._) (r⇚⊕ f)   = go (((A ⇛> B) <⇚ _) <⊢ _) f r⇚⊕
    find ((A ⇛> B) <⊢ ._) (d⇛⇐ f)   = go ((B <⊗ _) <⊢ _)        f d⇛⇐
    find ((A ⇛> B) <⊢ ._) (d⇛⇒ f)   = go ((_ ⊗> B) <⊢ _)        f d⇛⇒
    find ((A ⇚> B) <⊢ ._) (r⊗⇒ f)   = go ((_ ⊗> (A ⇚> B)) <⊢ _) f r⊗⇒
    find ((A ⇚> B) <⊢ ._) (r⊗⇐ f)   = go (((A ⇚> B) <⊗ _) <⊢ _) f r⊗⇐
    find ((A ⇚> B) <⊢ ._) (m⇚  f g) = go (_ ⊢> B)               g (m⇚ f)
    find ((A ⇚> B) <⊢ ._) (r⇛⊕ f)   = go ((_ ⇛> (A ⇚> B)) <⊢ _) f r⇛⊕
    find ((A ⇚> B) <⊢ ._) (r⊕⇚ f)   = go (_ ⊢> (_ ⊕> B))        f r⊕⇚
    find ((A ⇚> B) <⊢ ._) (r⇚⊕ f)   = go (((A ⇚> B) <⇚ _) <⊢ _) f r⇚⊕
    find ((A ⇚> B) <⊢ ._) (d⇚⇒ f)   = go (_ ⊢> (_ ⊕> B))        f d⇚⇒
    find ((A ⇚> B) <⊢ ._) (d⇚⇐ f)   = go (_ ⊢> (_ ⊕> B))        f d⇚⇐
    find ((A <⊗ B) <⊢ ._) (m⊗  f g) = go (A <⊢ _)               f (flip m⊗ g)
    find ((A <⊗ B) <⊢ ._) (r⇒⊗ f)   = go (_ ⊢> (A <⇒ _))        f r⇒⊗
    find ((A <⊗ B) <⊢ ._) (r⊗⇒ f)   = go ((_ ⊗> (A <⊗ B)) <⊢ _) f r⊗⇒
    find ((A <⊗ B) <⊢ ._) (r⇐⊗ f)   = go (A <⊢ _)               f r⇐⊗
    find ((A <⊗ B) <⊢ ._) (r⊗⇐ f)   = go (((A <⊗ B) <⊗ _) <⊢ _) f r⊗⇐
    find ((A <⊗ B) <⊢ ._) (r⇛⊕ f)   = go ((_ ⇛> (A <⊗ B)) <⊢ _) f r⇛⊕
    find ((A <⊗ B) <⊢ ._) (r⇚⊕ f)   = go (((A <⊗ B) <⇚ _) <⊢ _) f r⇚⊕
    find ((A <⇛ B) <⊢ ._) (r⊗⇒ f)   = go ((_ ⊗> (A <⇛ B)) <⊢ _) f r⊗⇒
    find ((A <⇛ B) <⊢ ._) (r⊗⇐ f)   = go (((A <⇛ B) <⊗ _) <⊢ _) f r⊗⇐
    find ((A <⇛ B) <⊢ ._) (m⇛  f g) = go (_ ⊢> A)               f (flip m⇛ g)
    find ((A <⇛ B) <⊢ ._) (r⇛⊕ f)   = go ((_ ⇛> (A <⇛ B)) <⊢ _) f r⇛⊕
    find ((A <⇛ B) <⊢ ._) (r⊕⇛ f)   = go (_ ⊢> (A <⊕ _))        f r⊕⇛
    find ((A <⇛ B) <⊢ ._) (r⇚⊕ f)   = go (((A <⇛ B) <⇚ _) <⊢ _) f r⇚⊕
    find ((A <⇛ B) <⊢ ._) (d⇛⇐ f)   = go (_ ⊢> (A <⊕ _))        f d⇛⇐
    find ((A <⇛ B) <⊢ ._) (d⇛⇒ f)   = go (_ ⊢> (A <⊕ _))        f d⇛⇒
    find ((A <⇚ B) <⊢ ._) (r⊗⇒ f)   = go ((_ ⊗> (A <⇚ B)) <⊢ _) f r⊗⇒
    find ((A <⇚ B) <⊢ ._) (r⊗⇐ f)   = go (((A <⇚ B) <⊗ _) <⊢ _) f r⊗⇐
    find ((A <⇚ B) <⊢ ._) (m⇚  f g) = go (A <⊢ _)               f (flip m⇚  g)
    find ((A <⇚ B) <⊢ ._) (r⇛⊕ f)   = go ((_ ⇛> (A <⇚ B)) <⊢ _) f r⇛⊕
    find ((A <⇚ B) <⊢ ._) (r⊕⇚ f)   = go (A <⊢ _)               f r⊕⇚
    find ((A <⇚ B) <⊢ ._) (r⇚⊕ f)   = go (((A <⇚ B) <⇚ _) <⊢ _) f r⇚⊕
    find ((A <⇚ B) <⊢ ._) (d⇚⇒ f)   = go ((_ ⊗> A) <⊢ _)        f d⇚⇒
    find ((A <⇚ B) <⊢ ._) (d⇚⇐ f)   = go ((A <⊗ _) <⊢ _)        f d⇚⇐
    find (._ ⊢> (A ⊕> B)) (r⇒⊗ f)   = go (_ ⊢> (_ ⇒> (A ⊕> B))) f r⇒⊗
    find (._ ⊢> (A ⊕> B)) (r⇐⊗ f)   = go (_ ⊢> ((A ⊕> B) <⇐ _)) f r⇐⊗
    find (._ ⊢> (A ⊕> B)) (m⊕  f g) = go (_ ⊢> B)               g (m⊕ f)
    find (._ ⊢> (A ⊕> B)) (r⇛⊕ f)   = go (_ ⊢> B)               f r⇛⊕
    find (._ ⊢> (A ⊕> B)) (r⊕⇛ f)   = go (_ ⊢> (_ ⊕> (A ⊕> B))) f r⊕⇛
    find (._ ⊢> (A ⊕> B)) (r⊕⇚ f)   = go (_ ⊢> ((A ⊕> B) <⊕ _)) f r⊕⇚
    find (._ ⊢> (A ⊕> B)) (r⇚⊕ f)   = go ((_ ⇚> B) <⊢ _)        f r⇚⊕
    find (._ ⊢> (A ⇒> B)) (m⇒  f g) = go (_ ⊢> B)               g (m⇒ f)
    find (._ ⊢> (A ⇒> B)) (r⇒⊗ f)   = go (_ ⊢> (_ ⇒> (A ⇒> B))) f r⇒⊗
    find (._ ⊢> (A ⇒> B)) (r⊗⇒ f)   = go (_ ⊢> B)               f r⊗⇒
    find (._ ⊢> (A ⇒> B)) (r⇐⊗ f)   = go (_ ⊢> ((A ⇒> B) <⇐ _)) f r⇐⊗
    find (._ ⊢> (A ⇒> B)) (r⊕⇛ f)   = go (_ ⊢> (_ ⊕> (A ⇒> B))) f r⊕⇛
    find (._ ⊢> (A ⇒> B)) (r⊕⇚ f)   = go (_ ⊢> ((A ⇒> B) <⊕ _)) f r⊕⇚
    find (._ ⊢> (A ⇒> B)) (d⇛⇒ f)   = go (_ ⊢> (_ ⊕> B))        f d⇛⇒
    find (._ ⊢> (A ⇒> B)) (d⇚⇒ f)   = go (_ ⊢> (B <⊕ _))        f d⇚⇒
    find (._ ⊢> (A ⇐> B)) (m⇐  f g) = go (B <⊢ _)               g (m⇐ f)
    find (._ ⊢> (A ⇐> B)) (r⇒⊗ f)   = go (_ ⊢> (_ ⇒> (A ⇐> B))) f r⇒⊗
    find (._ ⊢> (A ⇐> B)) (r⇐⊗ f)   = go (_ ⊢> ((A ⇐> B) <⇐ _)) f r⇐⊗
    find (._ ⊢> (A ⇐> B)) (r⊗⇐ f)   = go ((_ ⊗> B) <⊢ _)        f r⊗⇐
    find (._ ⊢> (A ⇐> B)) (r⊕⇛ f)   = go (_ ⊢> (_ ⊕> (A ⇐> B))) f r⊕⇛
    find (._ ⊢> (A ⇐> B)) (r⊕⇚ f)   = go (_ ⊢> ((A ⇐> B) <⊕ _)) f r⊕⇚
    find (._ ⊢> (A ⇐> B)) (d⇛⇐ f)   = go ((_ ⊗> B) <⊢ _)        f d⇛⇐
    find (._ ⊢> (A ⇐> B)) (d⇚⇐ f)   = go ((_ ⊗> B) <⊢ _)        f d⇚⇐
    find (._ ⊢> (A <⊕ B)) (r⇒⊗ f)   = go (_ ⊢> (_ ⇒> (A <⊕ B))) f r⇒⊗
    find (._ ⊢> (A <⊕ B)) (r⇐⊗ f)   = go (_ ⊢> ((A <⊕ B) <⇐ _)) f r⇐⊗
    find (._ ⊢> (A <⊕ B)) (m⊕  f g) = go (_ ⊢> A)               f (flip m⊕ g)
    find (._ ⊢> (A <⊕ B)) (r⇛⊕ f)   = go ((A <⇛ _) <⊢ _)        f r⇛⊕
    find (._ ⊢> (A <⊕ B)) (r⊕⇛ f)   = go (_ ⊢> (_ ⊕> (A <⊕ B))) f r⊕⇛
    find (._ ⊢> (A <⊕ B)) (r⊕⇚ f)   = go (_ ⊢> ((A <⊕ B) <⊕ _)) f r⊕⇚
    find (._ ⊢> (A <⊕ B)) (r⇚⊕ f)   = go (_ ⊢> A)               f r⇚⊕
    find (._ ⊢> (A <⇒ B)) (m⇒  f g) = go (A <⊢ _)               f (flip m⇒ g)
    find (._ ⊢> (A <⇒ B)) (r⇒⊗ f)   = go (_ ⊢> (_ ⇒> (A <⇒ B))) f r⇒⊗
    find (._ ⊢> (A <⇒ B)) (r⊗⇒ f)   = go ((A <⊗ _) <⊢ _)        f r⊗⇒
    find (._ ⊢> (A <⇒ B)) (r⇐⊗ f)   = go (_ ⊢> ((A <⇒ B) <⇐ _)) f r⇐⊗
    find (._ ⊢> (A <⇒ B)) (r⊕⇛ f)   = go (_ ⊢> (_ ⊕> (A <⇒ B))) f r⊕⇛
    find (._ ⊢> (A <⇒ B)) (r⊕⇚ f)   = go (_ ⊢> ((A <⇒ B) <⊕ _)) f r⊕⇚
    find (._ ⊢> (A <⇒ B)) (d⇛⇒ f)   = go ((A <⊗ _) <⊢ _)        f d⇛⇒
    find (._ ⊢> (A <⇒ B)) (d⇚⇒ f)   = go ((A <⊗ _) <⊢ _)        f d⇚⇒
    find (._ ⊢> (A <⇐ B)) (m⇐  f g) = go (_ ⊢> A)               f (flip m⇐ g)
    find (._ ⊢> (A <⇐ B)) (r⇒⊗ f)   = go (_ ⊢> (_ ⇒> (A <⇐ B))) f r⇒⊗
    find (._ ⊢> (A <⇐ B)) (r⇐⊗ f)   = go (_ ⊢> ((A <⇐ B) <⇐ _)) f r⇐⊗
    find (._ ⊢> (A <⇐ B)) (r⊗⇐ f)   = go (_ ⊢> A)               f r⊗⇐
    find (._ ⊢> (A <⇐ B)) (r⊕⇛ f)   = go (_ ⊢> (_ ⊕> (A <⇐ B))) f r⊕⇛
    find (._ ⊢> (A <⇐ B)) (r⊕⇚ f)   = go (_ ⊢> ((A <⇐ B) <⊕ _)) f r⊕⇚
    find (._ ⊢> (A <⇐ B)) (d⇛⇐ f)   = go (_ ⊢> (_ ⊕> A))        f d⇛⇐
    find (._ ⊢> (A <⇐ B)) (d⇚⇐ f)   = go (_ ⊢> (A <⊕ _))        f d⇚⇐

    private
      go : ∀ {B C}
         → ( I : Contextᴶ + ) (f : LG I [ B ⇐ C ]ᴶ)
         → { J : Contextᴶ + } (g : ∀ {G} → LG I [ G ]ᴶ → LG J [ G ]ᴶ)
         → Origin J (g f)
      go I f {J} g with find I f
      ... | origin h₁ h₂ f′ pr rewrite pr = origin h₁ h₂ (g ∘ f′) refl


module ⊕ where

  data Origin {B C} (J : Contextᴶ +) (f : LG J [ B ⊕ C ]ᴶ) : Set ℓ₁ where
    origin : ∀ {E F}  (h₁  : LG B ⊢ E)
              (h₂  : LG C ⊢ F)
              (f′  : ∀ {G} → LG G ⊢ E ⊕ F → LG J [ G ]ᴶ)
              (pr  : f ≡ f′ (m⊕ h₁ h₂))
                   → Origin J f

  mutual
    find : ∀ {B C} (J : Contextᴶ +) (f : LG J [ B ⊕ C ]ᴶ) → Origin J f
    find ([] <⊢ ._)       (m⊕  f g) = origin f g id refl
    find ([] <⊢ ._)       (r⊗⇒ f)   = go ((_ ⊗> []) <⊢ _)       f r⊗⇒
    find ([] <⊢ ._)       (r⊗⇐ f)   = go (([] <⊗ _) <⊢ _)       f r⊗⇐
    find ([] <⊢ ._)       (r⇛⊕ f)   = go ((_ ⇛> []) <⊢ _)       f r⇛⊕
    find ([] <⊢ ._)       (r⇚⊕ f)   = go (([] <⇚ _) <⊢ _)       f r⇚⊕
    find ((A ⊗> B) <⊢ ._) (m⊗  f g) = go (B <⊢ _)               g (m⊗ f)
    find ((A ⊗> B) <⊢ ._) (r⇒⊗ f)   = go (B <⊢ _)               f r⇒⊗
    find ((A ⊗> B) <⊢ ._) (r⊗⇒ f)   = go ((_ ⊗> (A ⊗> B)) <⊢ _) f r⊗⇒
    find ((A ⊗> B) <⊢ ._) (r⇐⊗ f)   = go (_ ⊢> (_ ⇐> B))        f r⇐⊗
    find ((A ⊗> B) <⊢ ._) (r⊗⇐ f)   = go (((A ⊗> B) <⊗ _) <⊢ _) f r⊗⇐
    find ((A ⊗> B) <⊢ ._) (r⇛⊕ f)   = go ((_ ⇛> (A ⊗> B)) <⊢ _) f r⇛⊕
    find ((A ⊗> B) <⊢ ._) (r⇚⊕ f)   = go (((A ⊗> B) <⇚ _) <⊢ _) f r⇚⊕
    find ((A ⇛> B) <⊢ ._) (r⊗⇒ f)   = go ((_ ⊗> (A ⇛> B)) <⊢ _) f r⊗⇒
    find ((A ⇛> B) <⊢ ._) (r⊗⇐ f)   = go (((A ⇛> B) <⊗ _) <⊢ _) f r⊗⇐
    find ((A ⇛> B) <⊢ ._) (m⇛  f g) = go (B <⊢ _)               g (m⇛ f)
    find ((A ⇛> B) <⊢ ._) (r⇛⊕ f)   = go ((_ ⇛> (A ⇛> B)) <⊢ _) f r⇛⊕
    find ((A ⇛> B) <⊢ ._) (r⊕⇛ f)   = go (B <⊢ _)               f r⊕⇛
    find ((A ⇛> B) <⊢ ._) (r⇚⊕ f)   = go (((A ⇛> B) <⇚ _) <⊢ _) f r⇚⊕
    find ((A ⇛> B) <⊢ ._) (d⇛⇐ f)   = go ((B <⊗ _) <⊢ _)        f d⇛⇐
    find ((A ⇛> B) <⊢ ._) (d⇛⇒ f)   = go ((_ ⊗> B) <⊢ _)        f d⇛⇒
    find ((A ⇚> B) <⊢ ._) (r⊗⇒ f)   = go ((_ ⊗> (A ⇚> B)) <⊢ _) f r⊗⇒
    find ((A ⇚> B) <⊢ ._) (r⊗⇐ f)   = go (((A ⇚> B) <⊗ _) <⊢ _) f r⊗⇐
    find ((A ⇚> B) <⊢ ._) (m⇚  f g) = go (_ ⊢> B)               g (m⇚ f)
    find ((A ⇚> B) <⊢ ._) (r⇛⊕ f)   = go ((_ ⇛> (A ⇚> B)) <⊢ _) f r⇛⊕
    find ((A ⇚> B) <⊢ ._) (r⊕⇚ f)   = go (_ ⊢> (_ ⊕> B))        f r⊕⇚
    find ((A ⇚> B) <⊢ ._) (r⇚⊕ f)   = go (((A ⇚> B) <⇚ _) <⊢ _) f r⇚⊕
    find ((A ⇚> B) <⊢ ._) (d⇚⇒ f)   = go (_ ⊢> (_ ⊕> B))        f d⇚⇒
    find ((A ⇚> B) <⊢ ._) (d⇚⇐ f)   = go (_ ⊢> (_ ⊕> B))        f d⇚⇐
    find ((A <⊗ B) <⊢ ._) (m⊗  f g) = go (A <⊢ _)               f (flip m⊗ g)
    find ((A <⊗ B) <⊢ ._) (r⇒⊗ f)   = go (_ ⊢> (A <⇒ _))        f r⇒⊗
    find ((A <⊗ B) <⊢ ._) (r⊗⇒ f)   = go ((_ ⊗> (A <⊗ B)) <⊢ _) f r⊗⇒
    find ((A <⊗ B) <⊢ ._) (r⇐⊗ f)   = go (A <⊢ _)               f r⇐⊗
    find ((A <⊗ B) <⊢ ._) (r⊗⇐ f)   = go (((A <⊗ B) <⊗ _) <⊢ _) f r⊗⇐
    find ((A <⊗ B) <⊢ ._) (r⇛⊕ f)   = go ((_ ⇛> (A <⊗ B)) <⊢ _) f r⇛⊕
    find ((A <⊗ B) <⊢ ._) (r⇚⊕ f)   = go (((A <⊗ B) <⇚ _) <⊢ _) f r⇚⊕
    find ((A <⇛ B) <⊢ ._) (r⊗⇒ f)   = go ((_ ⊗> (A <⇛ B)) <⊢ _) f r⊗⇒
    find ((A <⇛ B) <⊢ ._) (r⊗⇐ f)   = go (((A <⇛ B) <⊗ _) <⊢ _) f r⊗⇐
    find ((A <⇛ B) <⊢ ._) (m⇛  f g) = go (_ ⊢> A)               f (flip m⇛ g)
    find ((A <⇛ B) <⊢ ._) (r⇛⊕ f)   = go ((_ ⇛> (A <⇛ B)) <⊢ _) f r⇛⊕
    find ((A <⇛ B) <⊢ ._) (r⊕⇛ f)   = go (_ ⊢> (A <⊕ _))        f r⊕⇛
    find ((A <⇛ B) <⊢ ._) (r⇚⊕ f)   = go (((A <⇛ B) <⇚ _) <⊢ _) f r⇚⊕
    find ((A <⇛ B) <⊢ ._) (d⇛⇐ f)   = go (_ ⊢> (A <⊕ _))        f d⇛⇐
    find ((A <⇛ B) <⊢ ._) (d⇛⇒ f)   = go (_ ⊢> (A <⊕ _))        f d⇛⇒
    find ((A <⇚ B) <⊢ ._) (r⊗⇒ f)   = go ((_ ⊗> (A <⇚ B)) <⊢ _) f r⊗⇒
    find ((A <⇚ B) <⊢ ._) (r⊗⇐ f)   = go (((A <⇚ B) <⊗ _) <⊢ _) f r⊗⇐
    find ((A <⇚ B) <⊢ ._) (m⇚  f g) = go (A <⊢ _)               f (flip m⇚ g)
    find ((A <⇚ B) <⊢ ._) (r⇛⊕ f)   = go ((_ ⇛> (A <⇚ B)) <⊢ _) f r⇛⊕
    find ((A <⇚ B) <⊢ ._) (r⊕⇚ f)   = go (A <⊢ _)               f r⊕⇚
    find ((A <⇚ B) <⊢ ._) (r⇚⊕ f)   = go (((A <⇚ B) <⇚ _) <⊢ _) f r⇚⊕
    find ((A <⇚ B) <⊢ ._) (d⇚⇒ f)   = go ((_ ⊗> A) <⊢ _)        f d⇚⇒
    find ((A <⇚ B) <⊢ ._) (d⇚⇐ f)   = go ((A <⊗ _) <⊢ _)        f d⇚⇐
    find (._ ⊢> (A ⊕> B)) (r⇒⊗ f)   = go (_ ⊢> (_ ⇒> (A ⊕> B))) f r⇒⊗
    find (._ ⊢> (A ⊕> B)) (r⇐⊗ f)   = go (_ ⊢> ((A ⊕> B) <⇐ _)) f r⇐⊗
    find (._ ⊢> (A ⊕> B)) (m⊕  f g) = go (_ ⊢> B)               g (m⊕ f)
    find (._ ⊢> (A ⊕> B)) (r⇛⊕ f)   = go (_ ⊢> B)               f r⇛⊕
    find (._ ⊢> (A ⊕> B)) (r⊕⇛ f)   = go (_ ⊢> (_ ⊕> (A ⊕> B))) f r⊕⇛
    find (._ ⊢> (A ⊕> B)) (r⊕⇚ f)   = go (_ ⊢> ((A ⊕> B) <⊕ _)) f r⊕⇚
    find (._ ⊢> (A ⊕> B)) (r⇚⊕ f)   = go ((_ ⇚> B) <⊢ _)        f r⇚⊕
    find (._ ⊢> (A ⇒> B)) (m⇒  f g) = go (_ ⊢> B)               g (m⇒ f)
    find (._ ⊢> (A ⇒> B)) (r⇒⊗ f)   = go (_ ⊢> (_ ⇒> (A ⇒> B))) f r⇒⊗
    find (._ ⊢> (A ⇒> B)) (r⊗⇒ f)   = go (_ ⊢> B)               f r⊗⇒
    find (._ ⊢> (A ⇒> B)) (r⇐⊗ f)   = go (_ ⊢> ((A ⇒> B) <⇐ _)) f r⇐⊗
    find (._ ⊢> (A ⇒> B)) (r⊕⇛ f)   = go (_ ⊢> (_ ⊕> (A ⇒> B))) f r⊕⇛
    find (._ ⊢> (A ⇒> B)) (r⊕⇚ f)   = go (_ ⊢> ((A ⇒> B) <⊕ _)) f r⊕⇚
    find (._ ⊢> (A ⇒> B)) (d⇛⇒ f)   = go (_ ⊢> (_ ⊕> B))        f d⇛⇒
    find (._ ⊢> (A ⇒> B)) (d⇚⇒ f)   = go (_ ⊢> (B <⊕ _))        f d⇚⇒
    find (._ ⊢> (A ⇐> B)) (m⇐  f g) = go (B <⊢ _)               g (m⇐ f)
    find (._ ⊢> (A ⇐> B)) (r⇒⊗ f)   = go (_ ⊢> (_ ⇒> (A ⇐> B))) f r⇒⊗
    find (._ ⊢> (A ⇐> B)) (r⇐⊗ f)   = go (_ ⊢> ((A ⇐> B) <⇐ _)) f r⇐⊗
    find (._ ⊢> (A ⇐> B)) (r⊗⇐ f)   = go ((_ ⊗> B) <⊢ _)        f r⊗⇐
    find (._ ⊢> (A ⇐> B)) (r⊕⇛ f)   = go (_ ⊢> (_ ⊕> (A ⇐> B))) f r⊕⇛
    find (._ ⊢> (A ⇐> B)) (r⊕⇚ f)   = go (_ ⊢> ((A ⇐> B) <⊕ _)) f r⊕⇚
    find (._ ⊢> (A ⇐> B)) (d⇛⇐ f)   = go ((_ ⊗> B) <⊢ _)        f d⇛⇐
    find (._ ⊢> (A ⇐> B)) (d⇚⇐ f)   = go ((_ ⊗> B) <⊢ _)        f d⇚⇐
    find (._ ⊢> (A <⊕ B)) (r⇒⊗ f)   = go (_ ⊢> (_ ⇒> (A <⊕ B))) f r⇒⊗
    find (._ ⊢> (A <⊕ B)) (r⇐⊗ f)   = go (_ ⊢> ((A <⊕ B) <⇐ _)) f r⇐⊗
    find (._ ⊢> (A <⊕ B)) (m⊕  f g) = go (_ ⊢> A)               f (flip m⊕ g)
    find (._ ⊢> (A <⊕ B)) (r⇛⊕ f)   = go ((A <⇛ _) <⊢ _)        f r⇛⊕
    find (._ ⊢> (A <⊕ B)) (r⊕⇛ f)   = go (_ ⊢> (_ ⊕> (A <⊕ B))) f r⊕⇛
    find (._ ⊢> (A <⊕ B)) (r⊕⇚ f)   = go (_ ⊢> ((A <⊕ B) <⊕ _)) f r⊕⇚
    find (._ ⊢> (A <⊕ B)) (r⇚⊕ f)   = go (_ ⊢> A)               f r⇚⊕
    find (._ ⊢> (A <⇒ B)) (m⇒  f g) = go (A <⊢ _)               f (flip m⇒ g)
    find (._ ⊢> (A <⇒ B)) (r⇒⊗ f)   = go (_ ⊢> (_ ⇒> (A <⇒ B))) f r⇒⊗
    find (._ ⊢> (A <⇒ B)) (r⊗⇒ f)   = go ((A <⊗ _) <⊢ _)        f r⊗⇒
    find (._ ⊢> (A <⇒ B)) (r⇐⊗ f)   = go (_ ⊢> ((A <⇒ B) <⇐ _)) f r⇐⊗
    find (._ ⊢> (A <⇒ B)) (r⊕⇛ f)   = go (_ ⊢> (_ ⊕> (A <⇒ B))) f r⊕⇛
    find (._ ⊢> (A <⇒ B)) (r⊕⇚ f)   = go (_ ⊢> ((A <⇒ B) <⊕ _)) f r⊕⇚
    find (._ ⊢> (A <⇒ B)) (d⇛⇒ f)   = go ((A <⊗ _) <⊢ _)        f d⇛⇒
    find (._ ⊢> (A <⇒ B)) (d⇚⇒ f)   = go ((A <⊗ _) <⊢ _)        f d⇚⇒
    find (._ ⊢> (A <⇐ B)) (m⇐  f g) = go (_ ⊢> A)               f (flip m⇐ g)
    find (._ ⊢> (A <⇐ B)) (r⇒⊗ f)   = go (_ ⊢> (_ ⇒> (A <⇐ B))) f r⇒⊗
    find (._ ⊢> (A <⇐ B)) (r⇐⊗ f)   = go (_ ⊢> ((A <⇐ B) <⇐ _)) f r⇐⊗
    find (._ ⊢> (A <⇐ B)) (r⊗⇐ f)   = go (_ ⊢> A)               f r⊗⇐
    find (._ ⊢> (A <⇐ B)) (r⊕⇛ f)   = go (_ ⊢> (_ ⊕> (A <⇐ B))) f r⊕⇛
    find (._ ⊢> (A <⇐ B)) (r⊕⇚ f)   = go (_ ⊢> ((A <⇐ B) <⊕ _)) f r⊕⇚
    find (._ ⊢> (A <⇐ B)) (d⇛⇐ f)   = go (_ ⊢> (_ ⊕> A))        f d⇛⇐
    find (._ ⊢> (A <⇐ B)) (d⇚⇐ f)   = go (_ ⊢> (A <⊕ _))        f d⇚⇐

    private
      go : ∀ {B C}
         → ( I : Contextᴶ + ) (f : LG I [ B ⊕ C ]ᴶ)
         → { J : Contextᴶ + } (g : ∀ {G} → LG I [ G ]ᴶ → LG J [ G ]ᴶ)
         → Origin J (g f)
      go I f {J} g with find I f
      ... | origin h₁ h₂ f′ pr rewrite pr = origin h₁ h₂ (g ∘ f′) refl


module ⇚ where

  data Origin {B C} (J : Contextᴶ -) (f : LG J [ B ⇚ C ]ᴶ) : Set ℓ₁ where
    origin : ∀ {E F}  (h₁  : LG E ⊢ B)
              (h₂  : LG C ⊢ F)
              (f′  : ∀ {G} → LG E ⇚ F ⊢ G → LG J [ G ]ᴶ)
              (pr  : f ≡ f′ (m⇚ h₁ h₂))
                   → Origin J f

  mutual
    find : ∀ {B C} (J : Contextᴶ -) (f : LG J [ B ⇚ C ]ᴶ) → Origin J f
    find (._ ⊢> [])       (m⇚  f g) = origin f g id refl
    find (._ ⊢> [])       (r⇒⊗ f)   = go (_ ⊢> (_ ⇒> []))       f r⇒⊗
    find (._ ⊢> [])       (r⇐⊗ f)   = go (_ ⊢> ([] <⇐ _))       f r⇐⊗
    find (._ ⊢> [])       (r⊕⇛ f)   = go (_ ⊢> (_ ⊕> []))       f r⊕⇛
    find (._ ⊢> [])       (r⊕⇚ f)   = go (_ ⊢> ([] <⊕ _))       f r⊕⇚
    find ((A ⊗> B) <⊢ ._) (m⊗  f g) = go (B <⊢ _)               g (m⊗ f)
    find ((A ⊗> B) <⊢ ._) (r⇒⊗ f)   = go (B <⊢ _)               f r⇒⊗
    find ((A ⊗> B) <⊢ ._) (r⊗⇒ f)   = go ((_ ⊗> (A ⊗> B)) <⊢ _) f r⊗⇒
    find ((A ⊗> B) <⊢ ._) (r⇐⊗ f)   = go (_ ⊢> (_ ⇐> B))        f r⇐⊗
    find ((A ⊗> B) <⊢ ._) (r⊗⇐ f)   = go (((A ⊗> B) <⊗ _) <⊢ _) f r⊗⇐
    find ((A ⊗> B) <⊢ ._) (r⇛⊕ f)   = go ((_ ⇛> (A ⊗> B)) <⊢ _) f r⇛⊕
    find ((A ⊗> B) <⊢ ._) (r⇚⊕ f)   = go (((A ⊗> B) <⇚ _) <⊢ _) f r⇚⊕
    find ((A ⇛> B) <⊢ ._) (r⊗⇒ f)   = go ((_ ⊗> (A ⇛> B)) <⊢ _) f r⊗⇒
    find ((A ⇛> B) <⊢ ._) (r⊗⇐ f)   = go (((A ⇛> B) <⊗ _) <⊢ _) f r⊗⇐
    find ((A ⇛> B) <⊢ ._) (m⇛  f g) = go (B <⊢ _)               g (m⇛ f)
    find ((A ⇛> B) <⊢ ._) (r⇛⊕ f)   = go ((_ ⇛> (A ⇛> B)) <⊢ _) f r⇛⊕
    find ((A ⇛> B) <⊢ ._) (r⊕⇛ f)   = go (B <⊢ _)               f r⊕⇛
    find ((A ⇛> B) <⊢ ._) (r⇚⊕ f)   = go (((A ⇛> B) <⇚ _) <⊢ _) f r⇚⊕
    find ((A ⇛> B) <⊢ ._) (d⇛⇐ f)   = go ((B <⊗ _) <⊢ _)        f d⇛⇐
    find ((A ⇛> B) <⊢ ._) (d⇛⇒ f)   = go ((_ ⊗> B) <⊢ _)        f d⇛⇒
    find ((A ⇚> B) <⊢ ._) (r⊗⇒ f)   = go ((_ ⊗> (A ⇚> B)) <⊢ _) f r⊗⇒
    find ((A ⇚> B) <⊢ ._) (r⊗⇐ f)   = go (((A ⇚> B) <⊗ _) <⊢ _) f r⊗⇐
    find ((A ⇚> B) <⊢ ._) (m⇚  f g) = go (_ ⊢> B)               g (m⇚ f)
    find ((A ⇚> B) <⊢ ._) (r⇛⊕ f)   = go ((_ ⇛> (A ⇚> B)) <⊢ _) f r⇛⊕
    find ((A ⇚> B) <⊢ ._) (r⊕⇚ f)   = go (_ ⊢> (_ ⊕> B))        f r⊕⇚
    find ((A ⇚> B) <⊢ ._) (r⇚⊕ f)   = go (((A ⇚> B) <⇚ _) <⊢ _) f r⇚⊕
    find ((A ⇚> B) <⊢ ._) (d⇚⇒ f)   = go (_ ⊢> (_ ⊕> B))        f d⇚⇒
    find ((A ⇚> B) <⊢ ._) (d⇚⇐ f)   = go (_ ⊢> (_ ⊕> B))        f d⇚⇐
    find ((A <⊗ B) <⊢ ._) (m⊗  f g) = go (A <⊢ _)               f (flip m⊗ g)
    find ((A <⊗ B) <⊢ ._) (r⇒⊗ f)   = go (_ ⊢> (A <⇒ _))        f r⇒⊗
    find ((A <⊗ B) <⊢ ._) (r⊗⇒ f)   = go ((_ ⊗> (A <⊗ B)) <⊢ _) f r⊗⇒
    find ((A <⊗ B) <⊢ ._) (r⇐⊗ f)   = go (A <⊢ _)               f r⇐⊗
    find ((A <⊗ B) <⊢ ._) (r⊗⇐ f)   = go (((A <⊗ B) <⊗ _) <⊢ _) f r⊗⇐
    find ((A <⊗ B) <⊢ ._) (r⇛⊕ f)   = go ((_ ⇛> (A <⊗ B)) <⊢ _) f r⇛⊕
    find ((A <⊗ B) <⊢ ._) (r⇚⊕ f)   = go (((A <⊗ B) <⇚ _) <⊢ _) f r⇚⊕
    find ((A <⇛ B) <⊢ ._) (r⊗⇒ f)   = go ((_ ⊗> (A <⇛ B)) <⊢ _) f r⊗⇒
    find ((A <⇛ B) <⊢ ._) (r⊗⇐ f)   = go (((A <⇛ B) <⊗ _) <⊢ _) f r⊗⇐
    find ((A <⇛ B) <⊢ ._) (m⇛  f g) = go (_ ⊢> A)               f (flip m⇛ g)
    find ((A <⇛ B) <⊢ ._) (r⇛⊕ f)   = go ((_ ⇛> (A <⇛ B)) <⊢ _) f r⇛⊕
    find ((A <⇛ B) <⊢ ._) (r⊕⇛ f)   = go (_ ⊢> (A <⊕ _))        f r⊕⇛
    find ((A <⇛ B) <⊢ ._) (r⇚⊕ f)   = go (((A <⇛ B) <⇚ _) <⊢ _) f r⇚⊕
    find ((A <⇛ B) <⊢ ._) (d⇛⇐ f)   = go (_ ⊢> (A <⊕ _))        f d⇛⇐
    find ((A <⇛ B) <⊢ ._) (d⇛⇒ f)   = go (_ ⊢> (A <⊕ _))        f d⇛⇒
    find ((A <⇚ B) <⊢ ._) (r⊗⇒ f)   = go ((_ ⊗> (A <⇚ B)) <⊢ _) f r⊗⇒
    find ((A <⇚ B) <⊢ ._) (r⊗⇐ f)   = go (((A <⇚ B) <⊗ _) <⊢ _) f r⊗⇐
    find ((A <⇚ B) <⊢ ._) (m⇚  f g) = go (A <⊢ _)               f (flip m⇚ g)
    find ((A <⇚ B) <⊢ ._) (r⇛⊕ f)   = go ((_ ⇛> (A <⇚ B)) <⊢ _) f r⇛⊕
    find ((A <⇚ B) <⊢ ._) (r⊕⇚ f)   = go (A <⊢ _)               f r⊕⇚
    find ((A <⇚ B) <⊢ ._) (r⇚⊕ f)   = go (((A <⇚ B) <⇚ _) <⊢ _) f r⇚⊕
    find ((A <⇚ B) <⊢ ._) (d⇚⇒ f)   = go ((_ ⊗> A) <⊢ _)        f d⇚⇒
    find ((A <⇚ B) <⊢ ._) (d⇚⇐ f)   = go ((A <⊗ _) <⊢ _)        f d⇚⇐
    find (._ ⊢> (A ⊕> B)) (r⇒⊗ f)   = go (_ ⊢> (_ ⇒> (A ⊕> B))) f r⇒⊗
    find (._ ⊢> (A ⊕> B)) (r⇐⊗ f)   = go (_ ⊢> ((A ⊕> B) <⇐ _)) f r⇐⊗
    find (._ ⊢> (A ⊕> B)) (m⊕  f g) = go (_ ⊢> B)               g (m⊕ f)
    find (._ ⊢> (A ⊕> B)) (r⇛⊕ f)   = go (_ ⊢> B)               f r⇛⊕
    find (._ ⊢> (A ⊕> B)) (r⊕⇛ f)   = go (_ ⊢> (_ ⊕> (A ⊕> B))) f r⊕⇛
    find (._ ⊢> (A ⊕> B)) (r⊕⇚ f)   = go (_ ⊢> ((A ⊕> B) <⊕ _)) f r⊕⇚
    find (._ ⊢> (A ⊕> B)) (r⇚⊕ f)   = go ((_ ⇚> B) <⊢ _)        f r⇚⊕
    find (._ ⊢> (A ⇒> B)) (m⇒  f g) = go (_ ⊢> B)               g (m⇒ f)
    find (._ ⊢> (A ⇒> B)) (r⇒⊗ f)   = go (_ ⊢> (_ ⇒> (A ⇒> B))) f r⇒⊗
    find (._ ⊢> (A ⇒> B)) (r⊗⇒ f)   = go (_ ⊢> B)               f r⊗⇒
    find (._ ⊢> (A ⇒> B)) (r⇐⊗ f)   = go (_ ⊢> ((A ⇒> B) <⇐ _)) f r⇐⊗
    find (._ ⊢> (A ⇒> B)) (r⊕⇛ f)   = go (_ ⊢> (_ ⊕> (A ⇒> B))) f r⊕⇛
    find (._ ⊢> (A ⇒> B)) (r⊕⇚ f)   = go (_ ⊢> ((A ⇒> B) <⊕ _)) f r⊕⇚
    find (._ ⊢> (A ⇒> B)) (d⇛⇒ f)   = go (_ ⊢> (_ ⊕> B))        f d⇛⇒
    find (._ ⊢> (A ⇒> B)) (d⇚⇒ f)   = go (_ ⊢> (B <⊕ _))        f d⇚⇒
    find (._ ⊢> (A ⇐> B)) (m⇐  f g) = go (B <⊢ _)               g (m⇐ f)
    find (._ ⊢> (A ⇐> B)) (r⇒⊗ f)   = go (_ ⊢> (_ ⇒> (A ⇐> B))) f r⇒⊗
    find (._ ⊢> (A ⇐> B)) (r⇐⊗ f)   = go (_ ⊢> ((A ⇐> B) <⇐ _)) f r⇐⊗
    find (._ ⊢> (A ⇐> B)) (r⊗⇐ f)   = go ((_ ⊗> B) <⊢ _)        f r⊗⇐
    find (._ ⊢> (A ⇐> B)) (r⊕⇛ f)   = go (_ ⊢> (_ ⊕> (A ⇐> B))) f r⊕⇛
    find (._ ⊢> (A ⇐> B)) (r⊕⇚ f)   = go (_ ⊢> ((A ⇐> B) <⊕ _)) f r⊕⇚
    find (._ ⊢> (A ⇐> B)) (d⇛⇐ f)   = go ((_ ⊗> B) <⊢ _)        f d⇛⇐
    find (._ ⊢> (A ⇐> B)) (d⇚⇐ f)   = go ((_ ⊗> B) <⊢ _)        f d⇚⇐
    find (._ ⊢> (A <⊕ B)) (r⇒⊗ f)   = go (_ ⊢> (_ ⇒> (A <⊕ B))) f r⇒⊗
    find (._ ⊢> (A <⊕ B)) (r⇐⊗ f)   = go (_ ⊢> ((A <⊕ B) <⇐ _)) f r⇐⊗
    find (._ ⊢> (A <⊕ B)) (m⊕  f g) = go (_ ⊢> A)               f (flip m⊕ g)
    find (._ ⊢> (A <⊕ B)) (r⇛⊕ f)   = go ((A <⇛ _) <⊢ _)        f r⇛⊕
    find (._ ⊢> (A <⊕ B)) (r⊕⇛ f)   = go (_ ⊢> (_ ⊕> (A <⊕ B))) f r⊕⇛
    find (._ ⊢> (A <⊕ B)) (r⊕⇚ f)   = go (_ ⊢> ((A <⊕ B) <⊕ _)) f r⊕⇚
    find (._ ⊢> (A <⊕ B)) (r⇚⊕ f)   = go (_ ⊢> A)               f r⇚⊕
    find (._ ⊢> (A <⇒ B)) (m⇒  f g) = go (A <⊢ _)               f (flip m⇒ g)
    find (._ ⊢> (A <⇒ B)) (r⇒⊗ f)   = go (_ ⊢> (_ ⇒> (A <⇒ B))) f r⇒⊗
    find (._ ⊢> (A <⇒ B)) (r⊗⇒ f)   = go ((A <⊗ _) <⊢ _)        f r⊗⇒
    find (._ ⊢> (A <⇒ B)) (r⇐⊗ f)   = go (_ ⊢> ((A <⇒ B) <⇐ _)) f r⇐⊗
    find (._ ⊢> (A <⇒ B)) (r⊕⇛ f)   = go (_ ⊢> (_ ⊕> (A <⇒ B))) f r⊕⇛
    find (._ ⊢> (A <⇒ B)) (r⊕⇚ f)   = go (_ ⊢> ((A <⇒ B) <⊕ _)) f r⊕⇚
    find (._ ⊢> (A <⇒ B)) (d⇛⇒ f)   = go ((A <⊗ _) <⊢ _)        f d⇛⇒
    find (._ ⊢> (A <⇒ B)) (d⇚⇒ f)   = go ((A <⊗ _) <⊢ _)        f d⇚⇒
    find (._ ⊢> (A <⇐ B)) (m⇐  f g) = go (_ ⊢> A)               f (flip m⇐ g)
    find (._ ⊢> (A <⇐ B)) (r⇒⊗ f)   = go (_ ⊢> (_ ⇒> (A <⇐ B))) f r⇒⊗
    find (._ ⊢> (A <⇐ B)) (r⇐⊗ f)   = go (_ ⊢> ((A <⇐ B) <⇐ _)) f r⇐⊗
    find (._ ⊢> (A <⇐ B)) (r⊗⇐ f)   = go (_ ⊢> A)               f r⊗⇐
    find (._ ⊢> (A <⇐ B)) (r⊕⇛ f)   = go (_ ⊢> (_ ⊕> (A <⇐ B))) f r⊕⇛
    find (._ ⊢> (A <⇐ B)) (r⊕⇚ f)   = go (_ ⊢> ((A <⇐ B) <⊕ _)) f r⊕⇚
    find (._ ⊢> (A <⇐ B)) (d⇛⇐ f)   = go (_ ⊢> (_ ⊕> A))        f d⇛⇐
    find (._ ⊢> (A <⇐ B)) (d⇚⇐ f)   = go (_ ⊢> (A <⊕ _))        f d⇚⇐

    private
      go : ∀ {B C}
         → ( I : Contextᴶ - ) (f : LG I [ B ⇚ C ]ᴶ)
         → { J : Contextᴶ - } (g : ∀ {G} → LG I [ G ]ᴶ → LG J [ G ]ᴶ)
         → Origin J (g f)
      go I f {J} g with find I f
      ... | origin h₁ h₂ f′ pr rewrite pr = origin h₁ h₂ (g ∘ f′) refl


module ⇛ where

  data Origin {B C} (J : Contextᴶ -) (f : LG J [ B ⇛ C ]ᴶ) : Set ℓ₁ where
    origin : ∀ {E F}  (h₁   : LG B ⊢ E)
              (h₂   : LG F ⊢ C)
              (f′   : ∀ {G} → LG E ⇛ F ⊢ G → LG J [ G ]ᴶ)
              (pr   : f ≡ f′ (m⇛ h₁ h₂))
                   → Origin J f

  mutual
    find : ∀ {B C} (J : Contextᴶ -) (f : LG J [ B ⇛ C ]ᴶ) → Origin J f
    find (._ ⊢> [])       (m⇛  f g) = origin f g id refl
    find (._ ⊢> [])       (r⇒⊗ f)   = go (_ ⊢> (_ ⇒> []))       f r⇒⊗
    find (._ ⊢> [])       (r⇐⊗ f)   = go (_ ⊢> ([] <⇐ _))       f r⇐⊗
    find (._ ⊢> [])       (r⊕⇛ f)   = go (_ ⊢> (_ ⊕> []))       f r⊕⇛
    find (._ ⊢> [])       (r⊕⇚ f)   = go (_ ⊢> ([] <⊕ _))       f r⊕⇚
    find ((A ⊗> B) <⊢ ._) (m⊗  f g) = go (B <⊢ _)               g (m⊗ f)
    find ((A ⊗> B) <⊢ ._) (r⇒⊗ f)   = go (B <⊢ _)               f r⇒⊗
    find ((A ⊗> B) <⊢ ._) (r⊗⇒ f)   = go ((_ ⊗> (A ⊗> B)) <⊢ _) f r⊗⇒
    find ((A ⊗> B) <⊢ ._) (r⇐⊗ f)   = go (_ ⊢> (_ ⇐> B))        f r⇐⊗
    find ((A ⊗> B) <⊢ ._) (r⊗⇐ f)   = go (((A ⊗> B) <⊗ _) <⊢ _) f r⊗⇐
    find ((A ⊗> B) <⊢ ._) (r⇛⊕ f)   = go ((_ ⇛> (A ⊗> B)) <⊢ _) f r⇛⊕
    find ((A ⊗> B) <⊢ ._) (r⇚⊕ f)   = go (((A ⊗> B) <⇚ _) <⊢ _) f r⇚⊕
    find ((A ⇛> B) <⊢ ._) (r⊗⇒ f)   = go ((_ ⊗> (A ⇛> B)) <⊢ _) f r⊗⇒
    find ((A ⇛> B) <⊢ ._) (r⊗⇐ f)   = go (((A ⇛> B) <⊗ _) <⊢ _) f r⊗⇐
    find ((A ⇛> B) <⊢ ._) (m⇛  f g) = go (B <⊢ _)               g (m⇛ f)
    find ((A ⇛> B) <⊢ ._) (r⇛⊕ f)   = go ((_ ⇛> (A ⇛> B)) <⊢ _) f r⇛⊕
    find ((A ⇛> B) <⊢ ._) (r⊕⇛ f)   = go (B <⊢ _)               f r⊕⇛
    find ((A ⇛> B) <⊢ ._) (r⇚⊕ f)   = go (((A ⇛> B) <⇚ _) <⊢ _) f r⇚⊕
    find ((A ⇛> B) <⊢ ._) (d⇛⇐ f)   = go ((B <⊗ _) <⊢ _)        f d⇛⇐
    find ((A ⇛> B) <⊢ ._) (d⇛⇒ f)   = go ((_ ⊗> B) <⊢ _)        f d⇛⇒
    find ((A ⇚> B) <⊢ ._) (r⊗⇒ f)   = go ((_ ⊗> (A ⇚> B)) <⊢ _) f r⊗⇒
    find ((A ⇚> B) <⊢ ._) (r⊗⇐ f)   = go (((A ⇚> B) <⊗ _) <⊢ _) f r⊗⇐
    find ((A ⇚> B) <⊢ ._) (m⇚  f g) = go (_ ⊢> B)               g (m⇚ f)
    find ((A ⇚> B) <⊢ ._) (r⇛⊕ f)   = go ((_ ⇛> (A ⇚> B)) <⊢ _) f r⇛⊕
    find ((A ⇚> B) <⊢ ._) (r⊕⇚ f)   = go (_ ⊢> (_ ⊕> B))        f r⊕⇚
    find ((A ⇚> B) <⊢ ._) (r⇚⊕ f)   = go (((A ⇚> B) <⇚ _) <⊢ _) f r⇚⊕
    find ((A ⇚> B) <⊢ ._) (d⇚⇒ f)   = go (_ ⊢> (_ ⊕> B))        f d⇚⇒
    find ((A ⇚> B) <⊢ ._) (d⇚⇐ f)   = go (_ ⊢> (_ ⊕> B))        f d⇚⇐
    find ((A <⊗ B) <⊢ ._) (m⊗  f g) = go (A <⊢ _)               f (flip m⊗ g)
    find ((A <⊗ B) <⊢ ._) (r⇒⊗ f)   = go (_ ⊢> (A <⇒ _))        f r⇒⊗
    find ((A <⊗ B) <⊢ ._) (r⊗⇒ f)   = go ((_ ⊗> (A <⊗ B)) <⊢ _) f r⊗⇒
    find ((A <⊗ B) <⊢ ._) (r⇐⊗ f)   = go (A <⊢ _)               f r⇐⊗
    find ((A <⊗ B) <⊢ ._) (r⊗⇐ f)   = go (((A <⊗ B) <⊗ _) <⊢ _) f r⊗⇐
    find ((A <⊗ B) <⊢ ._) (r⇛⊕ f)   = go ((_ ⇛> (A <⊗ B)) <⊢ _) f r⇛⊕
    find ((A <⊗ B) <⊢ ._) (r⇚⊕ f)   = go (((A <⊗ B) <⇚ _) <⊢ _) f r⇚⊕
    find ((A <⇛ B) <⊢ ._) (r⊗⇒ f)   = go ((_ ⊗> (A <⇛ B)) <⊢ _) f r⊗⇒
    find ((A <⇛ B) <⊢ ._) (r⊗⇐ f)   = go (((A <⇛ B) <⊗ _) <⊢ _) f r⊗⇐
    find ((A <⇛ B) <⊢ ._) (m⇛  f g) = go (_ ⊢> A)               f (flip m⇛ g)
    find ((A <⇛ B) <⊢ ._) (r⇛⊕ f)   = go ((_ ⇛> (A <⇛ B)) <⊢ _) f r⇛⊕
    find ((A <⇛ B) <⊢ ._) (r⊕⇛ f)   = go (_ ⊢> (A <⊕ _))        f r⊕⇛
    find ((A <⇛ B) <⊢ ._) (r⇚⊕ f)   = go (((A <⇛ B) <⇚ _) <⊢ _) f r⇚⊕
    find ((A <⇛ B) <⊢ ._) (d⇛⇐ f)   = go (_ ⊢> (A <⊕ _))        f d⇛⇐
    find ((A <⇛ B) <⊢ ._) (d⇛⇒ f)   = go (_ ⊢> (A <⊕ _))        f d⇛⇒
    find ((A <⇚ B) <⊢ ._) (r⊗⇒ f)   = go ((_ ⊗> (A <⇚ B)) <⊢ _) f r⊗⇒
    find ((A <⇚ B) <⊢ ._) (r⊗⇐ f)   = go (((A <⇚ B) <⊗ _) <⊢ _) f r⊗⇐
    find ((A <⇚ B) <⊢ ._) (m⇚  f g) = go (A <⊢ _)               f (flip m⇚ g)
    find ((A <⇚ B) <⊢ ._) (r⇛⊕ f)   = go ((_ ⇛> (A <⇚ B)) <⊢ _) f r⇛⊕
    find ((A <⇚ B) <⊢ ._) (r⊕⇚ f)   = go (A <⊢ _)               f r⊕⇚
    find ((A <⇚ B) <⊢ ._) (r⇚⊕ f)   = go (((A <⇚ B) <⇚ _) <⊢ _) f r⇚⊕
    find ((A <⇚ B) <⊢ ._) (d⇚⇒ f)   = go ((_ ⊗> A) <⊢ _)        f d⇚⇒
    find ((A <⇚ B) <⊢ ._) (d⇚⇐ f)   = go ((A <⊗ _) <⊢ _)        f d⇚⇐
    find (._ ⊢> (A ⊕> B)) (r⇒⊗ f)   = go (_ ⊢> (_ ⇒> (A ⊕> B))) f r⇒⊗
    find (._ ⊢> (A ⊕> B)) (r⇐⊗ f)   = go (_ ⊢> ((A ⊕> B) <⇐ _)) f r⇐⊗
    find (._ ⊢> (A ⊕> B)) (m⊕  f g) = go (_ ⊢> B)               g (m⊕ f)
    find (._ ⊢> (A ⊕> B)) (r⇛⊕ f)   = go (_ ⊢> B)               f r⇛⊕
    find (._ ⊢> (A ⊕> B)) (r⊕⇛ f)   = go (_ ⊢> (_ ⊕> (A ⊕> B))) f r⊕⇛
    find (._ ⊢> (A ⊕> B)) (r⊕⇚ f)   = go (_ ⊢> ((A ⊕> B) <⊕ _)) f r⊕⇚
    find (._ ⊢> (A ⊕> B)) (r⇚⊕ f)   = go ((_ ⇚> B) <⊢ _)        f r⇚⊕
    find (._ ⊢> (A ⇒> B)) (m⇒  f g) = go (_ ⊢> B)               g (m⇒ f)
    find (._ ⊢> (A ⇒> B)) (r⇒⊗ f)   = go (_ ⊢> (_ ⇒> (A ⇒> B))) f r⇒⊗
    find (._ ⊢> (A ⇒> B)) (r⊗⇒ f)   = go (_ ⊢> B)               f r⊗⇒
    find (._ ⊢> (A ⇒> B)) (r⇐⊗ f)   = go (_ ⊢> ((A ⇒> B) <⇐ _)) f r⇐⊗
    find (._ ⊢> (A ⇒> B)) (r⊕⇛ f)   = go (_ ⊢> (_ ⊕> (A ⇒> B))) f r⊕⇛
    find (._ ⊢> (A ⇒> B)) (r⊕⇚ f)   = go (_ ⊢> ((A ⇒> B) <⊕ _)) f r⊕⇚
    find (._ ⊢> (A ⇒> B)) (d⇛⇒ f)   = go (_ ⊢> (_ ⊕> B))        f d⇛⇒
    find (._ ⊢> (A ⇒> B)) (d⇚⇒ f)   = go (_ ⊢> (B <⊕ _))        f d⇚⇒
    find (._ ⊢> (A ⇐> B)) (m⇐  f g) = go (B <⊢ _)               g (m⇐ f)
    find (._ ⊢> (A ⇐> B)) (r⇒⊗ f)   = go (_ ⊢> (_ ⇒> (A ⇐> B))) f r⇒⊗
    find (._ ⊢> (A ⇐> B)) (r⇐⊗ f)   = go (_ ⊢> ((A ⇐> B) <⇐ _)) f r⇐⊗
    find (._ ⊢> (A ⇐> B)) (r⊗⇐ f)   = go ((_ ⊗> B) <⊢ _)        f r⊗⇐
    find (._ ⊢> (A ⇐> B)) (r⊕⇛ f)   = go (_ ⊢> (_ ⊕> (A ⇐> B))) f r⊕⇛
    find (._ ⊢> (A ⇐> B)) (r⊕⇚ f)   = go (_ ⊢> ((A ⇐> B) <⊕ _)) f r⊕⇚
    find (._ ⊢> (A ⇐> B)) (d⇛⇐ f)   = go ((_ ⊗> B) <⊢ _)        f d⇛⇐
    find (._ ⊢> (A ⇐> B)) (d⇚⇐ f)   = go ((_ ⊗> B) <⊢ _)        f d⇚⇐
    find (._ ⊢> (A <⊕ B)) (r⇒⊗ f)   = go (_ ⊢> (_ ⇒> (A <⊕ B))) f r⇒⊗
    find (._ ⊢> (A <⊕ B)) (r⇐⊗ f)   = go (_ ⊢> ((A <⊕ B) <⇐ _)) f r⇐⊗
    find (._ ⊢> (A <⊕ B)) (m⊕  f g) = go (_ ⊢> A)               f (flip m⊕ g)
    find (._ ⊢> (A <⊕ B)) (r⇛⊕ f)   = go ((A <⇛ _) <⊢ _)        f r⇛⊕
    find (._ ⊢> (A <⊕ B)) (r⊕⇛ f)   = go (_ ⊢> (_ ⊕> (A <⊕ B))) f r⊕⇛
    find (._ ⊢> (A <⊕ B)) (r⊕⇚ f)   = go (_ ⊢> ((A <⊕ B) <⊕ _)) f r⊕⇚
    find (._ ⊢> (A <⊕ B)) (r⇚⊕ f)   = go (_ ⊢> A)               f r⇚⊕
    find (._ ⊢> (A <⇒ B)) (m⇒  f g) = go (A <⊢ _)               f (flip m⇒ g)
    find (._ ⊢> (A <⇒ B)) (r⇒⊗ f)   = go (_ ⊢> (_ ⇒> (A <⇒ B))) f r⇒⊗
    find (._ ⊢> (A <⇒ B)) (r⊗⇒ f)   = go ((A <⊗ _) <⊢ _)        f r⊗⇒
    find (._ ⊢> (A <⇒ B)) (r⇐⊗ f)   = go (_ ⊢> ((A <⇒ B) <⇐ _)) f r⇐⊗
    find (._ ⊢> (A <⇒ B)) (r⊕⇛ f)   = go (_ ⊢> (_ ⊕> (A <⇒ B))) f r⊕⇛
    find (._ ⊢> (A <⇒ B)) (r⊕⇚ f)   = go (_ ⊢> ((A <⇒ B) <⊕ _)) f r⊕⇚
    find (._ ⊢> (A <⇒ B)) (d⇛⇒ f)   = go ((A <⊗ _) <⊢ _)        f d⇛⇒
    find (._ ⊢> (A <⇒ B)) (d⇚⇒ f)   = go ((A <⊗ _) <⊢ _)        f d⇚⇒
    find (._ ⊢> (A <⇐ B)) (m⇐  f g) = go (_ ⊢> A)               f (flip m⇐ g)
    find (._ ⊢> (A <⇐ B)) (r⇒⊗ f)   = go (_ ⊢> (_ ⇒> (A <⇐ B))) f r⇒⊗
    find (._ ⊢> (A <⇐ B)) (r⇐⊗ f)   = go (_ ⊢> ((A <⇐ B) <⇐ _)) f r⇐⊗
    find (._ ⊢> (A <⇐ B)) (r⊗⇐ f)   = go (_ ⊢> A)               f r⊗⇐
    find (._ ⊢> (A <⇐ B)) (r⊕⇛ f)   = go (_ ⊢> (_ ⊕> (A <⇐ B))) f r⊕⇛
    find (._ ⊢> (A <⇐ B)) (r⊕⇚ f)   = go (_ ⊢> ((A <⇐ B) <⊕ _)) f r⊕⇚
    find (._ ⊢> (A <⇐ B)) (d⇛⇐ f)   = go (_ ⊢> (_ ⊕> A))        f d⇛⇐
    find (._ ⊢> (A <⇐ B)) (d⇚⇐ f)   = go (_ ⊢> (A <⊕ _))        f d⇚⇐

    private
      go : ∀ {B C}
         → ( I : Contextᴶ - ) (f : LG I [ B ⇛ C ]ᴶ)
         → { J : Contextᴶ - } (g : ∀ {G} → LG I [ G ]ᴶ → LG J [ G ]ᴶ)
         → Origin J (g f)
      go I f {J} g with find I f
      ... | origin h₁ h₂ f′ pr rewrite pr = origin h₁ h₂ (g ∘ f′) refl


trans′ : ∀ {A B C} (f : LG A ⊢ B) (g : LG B ⊢ C) → LG A ⊢ C
trans′ {B = el _ }  f  g with el.find ([] <⊢ _) g
... | (el.origin        g′ pr)  = g′ f
trans′ {B = _ ⊗ _}  f  g with ⊗.find (_ ⊢> []) f
... | (⊗.origin  h₁ h₂  f′ pr)  = f′ (r⇐⊗ (trans′ h₁ (r⊗⇐ (r⇒⊗ (trans′ h₂ (r⊗⇒ g))))))
trans′ {B = _ ⇐ _}  f  g with ⇐.find ([] <⊢ _) g
... | (⇐.origin  h₁ h₂  g′ pr)  = g′ (r⊗⇐ (r⇒⊗ (trans′ h₂ (r⊗⇒ (trans′ (r⇐⊗ f) h₁)))))
trans′ {B = _ ⇒ _}  f  g with ⇒.find ([] <⊢ _) g
... | (⇒.origin  h₁ h₂  g′ pr)  = g′ (r⊗⇒ (r⇐⊗ (trans′ h₁ (r⊗⇐ (trans′ (r⇒⊗ f) h₂)))))
trans′ {B = _ ⊕ _}  f  g with ⊕.find ([] <⊢ _) g
... | (⊕.origin  h₁ h₂  g′ pr)  = g′ (r⇚⊕ (trans′ (r⊕⇚ (r⇛⊕ (trans′ (r⊕⇛ f) h₂))) h₁))
trans′ {B = _ ⇚ _}  f  g with ⇚.find (_ ⊢> []) f
... | (⇚.origin  h₁ h₂  f′ pr)  = f′ (r⊕⇚ (r⇛⊕ (trans′ (r⊕⇛ (trans′ h₁ (r⇚⊕ g))) h₂)))
trans′ {B = _ ⇛ _}  f  g with ⇛.find (_ ⊢> []) f
... | (⇛.origin  h₁ h₂  f′ pr)  = f′ (r⊕⇛ (r⇚⊕ (trans′ (r⊕⇚ (trans′ h₂ (r⇛⊕ g))) h₁)))


⌈_⌉ : Type → Set ℓ₂
⌈ el  A ⌉ = ⟦ A ⟧
⌈ A ⊗ B ⌉ = ¬ (¬ (⌈ A ⌉ × ⌈ B ⌉))
⌈ A ⊕ B ⌉ = ¬ (¬ (⌈ A ⌉ ⊎ ⌈ B ⌉))
⌈ A ⇒ B ⌉ =    ¬ ⌈ B ⌉ → ¬ ⌈ A ⌉
⌈ B ⇐ A ⌉ =    ¬ ⌈ B ⌉ → ¬ ⌈ A ⌉
⌈ B ⇚ A ⌉ = ¬ (¬ ⌈ B ⌉ → ¬ ⌈ A ⌉)
⌈ A ⇛ B ⌉ = ¬ (¬ ⌈ B ⌉ → ¬ ⌈ A ⌉)
